theories/stacked_borrows/defs.v
@@ -1,0 +1,63 @@
+From simuliris.stacked_borrows Require Export class_instances tactics notation lang bor_semantics.
+
+
+
+Definition wf_mem_tag (h: mem) (nxtp: ptr_id) :=
+  ∀ l l' pid, h !! l = Some (ScPtr l' (Tagged pid)) → (pid < nxtp)%nat.
+
+Definition stack_item_included (stk: stack) (nxtp: ptr_id) (nxtc: call_id) :=
+  ∀ si, si ∈ stk → match si.(tg) with
+                    | Tagged t => (t < nxtp)%nat
+                    | _ => True
+                   end ∧
+                   match si.(protector) with
+                    | Some c => (c < nxtc)%nat
+                    | _ => True
+                   end.
+
+Definition is_tagged (it: item) :=
+  match it.(tg) with Tagged _ => True | _ => False end.
+Instance is_tagged_dec it: Decision (is_tagged it).
+Proof. intros. rewrite /is_tagged. case tg; solve_decision. Defined.
+Definition stack_item_tagged_NoDup (stk : stack) :=
+  NoDup (fmap tg (filter is_tagged stk)).
+
+Definition wf_stack (stk: stack) (nxtp: ptr_id) (nxtc: call_id) :=
+  stack_item_included stk nxtp nxtc ∧ stack_item_tagged_NoDup stk.
+Definition wf_stacks (α: stacks) (nxtp: ptr_id) (nxtc: call_id) :=
+  ∀ l stk, α !! l = Some stk → wf_stack stk nxtp nxtc.
+Definition wf_non_empty (α: stacks) :=
+  ∀ l stk, α !! l = Some stk → stk ≠ [].
+Definition wf_no_dup (α: stacks) :=
+  ∀ l stk, α !! l = Some stk → NoDup stk.
+Definition wf_cid_incl (cids: call_id_set) (nxtc: call_id) :=
+  ∀ c : call_id, c ∈ cids → (c < nxtc)%nat.
+Definition wf_scalar σ sc := ∀ t l, sc = ScPtr l t → t <t σ.(snp).
+
+Record state_wf (s: state) := {
+  state_wf_dom : dom (gset loc) s.(shp) ≡ dom (gset loc) s.(sst);
+  state_wf_mem_tag : wf_mem_tag s.(shp) s.(snp);
+  state_wf_stack_item : wf_stacks s.(sst) s.(snp) s.(snc);
+  state_wf_non_empty : wf_non_empty s.(sst);
+  (*state_wf_cid_no_dup : NoDup s.(scs) ;*)
+  state_wf_cid_agree: wf_cid_incl s.(scs) s.(snc);
+  (* state_wf_cid_non_empty : s.(scs) ≠ []; *)
+  (* state_wf_no_dup : wf_no_dup σ.(cst).(sst); *)
+}.
+
+Fixpoint active_SRO (stk: stack) : gset ptr_id :=
+  match stk with
+  | [] => ∅
+  | it :: stk =>
+    match it.(perm) with
+    | SharedReadOnly => match it.(tg) with
+                        | Tagged t => {[t]} ∪ active_SRO stk
+                        | Untagged => active_SRO stk
+                        end
+    | _ => ∅
+    end
+  end.
+
+
+Definition init_state := (mkState ∅ ∅ {[O]} O 1).
+
