theories/stacked_borrows/steps_retag.v
@@ -1,0 +1,1789 @@
+From simuliris.stacked_borrows Require Export defs steps_foreach steps_list steps_wf steps_progress.
+
+Set Default Proof Using "Type".
+
+Definition tag_on_top (stks: stacks) l t pm : Prop :=
+  ∃ prot, (stks !! l) ≫= head = Some (mkItem pm (Tagged t) prot).
+
+(** Active protector preserving *)
+Definition active_preserving (cids: call_id_set) (stk stk': stack) :=
+  ∀ pm t c, c ∈ cids → mkItem pm t (Some c) ∈ stk → mkItem pm t (Some c) ∈ stk'.
+
+Instance active_preserving_preorder cids : PreOrder (active_preserving cids).
+Proof.
+  constructor.
+  - intros ??. done.
+  - intros ??? AS1 AS2 ?????. naive_solver.
+Qed.
+
+Lemma active_preserving_app_mono (cids: call_id_set) (stk1 stk2 stk': stack) :
+  active_preserving cids stk1 stk2 →
+  active_preserving cids (stk1 ++ stk') (stk2 ++ stk').
+Proof.
+  intros AS pm t c Inc. rewrite 2!elem_of_app.
+  specialize (AS pm t c Inc). set_solver.
+Qed.
+
+Lemma remove_check_active_preserving cids stk stk' idx:
+  remove_check cids stk idx = Some stk' → active_preserving cids stk stk'.
+Proof.
+  revert idx.
+  induction stk as [|it stk IH]; intros idx; simpl.
+  { destruct idx; [|done]. intros ??. by simplify_eq. }
+  destruct idx as [|idx]; [intros ??; by simplify_eq|].
+  case check_protector eqn:Eq; [|done].
+  move => /IH AS pm t c IN /elem_of_cons [?|]; [|by apply AS].
+  subst it. exfalso. move : Eq.
+  by rewrite /check_protector /= /is_active bool_decide_true //.
+Qed.
+
+Lemma replace_check'_active_preserving cids acc stk stk':
+  replace_check' cids acc stk = Some stk' → active_preserving cids stk stk'.
+Proof.
+  revert acc.
+  induction stk as [|it stk IH]; intros acc; simpl.
+  { intros. simplify_eq. by intros ?????%not_elem_of_nil. }
+  case decide => ?; [case check_protector eqn:Eq; [|done]|].
+  - move => /IH AS pm t c IN /elem_of_cons [?|]; [|by apply AS].
+    subst it. exfalso. move : Eq.
+    by rewrite /check_protector /= /is_active bool_decide_true //.
+  - move => Eq pm t c IN /elem_of_cons [?|].
+    + apply (replace_check'_acc_result _ _ _ _ Eq), elem_of_app. right.
+      by apply elem_of_list_singleton.
+    + by apply (IH _ Eq).
+Qed.
+
+Lemma replace_check_active_preserving cids stk stk':
+  replace_check cids stk = Some stk' → active_preserving cids stk stk'.
+Proof. by apply replace_check'_active_preserving. Qed.
+
+Lemma access1_active_preserving stk stk' kind tg cids n:
+  access1 stk kind tg cids = Some (n, stk') →
+  active_preserving cids stk stk'.
+Proof.
+  rewrite /access1. case find_granting as [gip|]; [|done]. simpl.
+  destruct kind.
+  - case replace_check as [stk1|] eqn:Eq; [|done].
+    simpl. intros. simplify_eq.
+    rewrite -{1}(take_drop gip.1 stk).
+    by apply active_preserving_app_mono, replace_check_active_preserving.
+  - case find_first_write_incompatible as [idx|]; [|done]. simpl.
+    case remove_check as [stk1|] eqn:Eq; [|done].
+    simpl. intros. simplify_eq.
+    rewrite -{1}(take_drop gip.1 stk).
+    by eapply active_preserving_app_mono, remove_check_active_preserving.
+Qed.
+
+Lemma for_each_access1_active_preserving α cids l n tg kind α':
+  for_each α l n false
+          (λ stk, nstk' ← access1 stk kind tg cids; Some nstk'.2) = Some α' →
+  ∀ l stk, α !! l = Some stk →
+  ∃ stk', α' !! l = Some stk' ∧ active_preserving cids stk stk'.
+Proof.
+  intros EQ. destruct (for_each_lookup  _ _ _ _ _ EQ) as [EQ1 [EQ2 EQ3]].
+  intros l1 stk1 Eq1.
+  case (decide (l1.1 = l.1)) => [Eql|NEql];
+    [case (decide (l.2 ≤ l1.2 < l.2 + n)) => [[Le Lt]|NIN]|].
+  - have Eql2: l1 = l +ₗ Z.of_nat (Z.to_nat (l1.2 - l.2)). {
+      destruct l, l1. move : Eql Le => /= -> ?.
+      rewrite /shift_loc /= Z2Nat.id; [|lia]. f_equal. lia. }
+    destruct (EQ1 (Z.to_nat (l1.2 - l.2)) stk1)
+      as [stk [Eq [[n1 stk'] [Eq' Eq0]]%bind_Some]];
+      [rewrite -(Nat2Z.id n) -Z2Nat.inj_lt; lia|by rewrite -Eql2|].
+    exists stk. rewrite -Eql2 in Eq. split; [done|]. simpl in Eq0. simplify_eq.
+    eapply access1_active_preserving; eauto.
+  - rewrite EQ3; [naive_solver|].
+    intros i Lt Eq. apply NIN. rewrite Eq /=. lia.
+  - rewrite EQ3; [naive_solver|].
+    intros i Lt Eq. apply NEql. by rewrite Eq.
+Qed.
+
+Lemma for_each_access1_lookup_inv α cids l n tg kind α':
+  for_each α l n false
+          (λ stk, nstk' ← access1 stk kind tg cids; Some nstk'.2) = Some α' →
+  ∀ l stk, α !! l = Some stk →
+  ∃ stk', α' !! l = Some stk' ∧
+    ((∃ n', access1 stk kind tg cids = Some (n', stk')) ∨  α' !! l = α !! l).
+Proof.
+  intros EQ. destruct (for_each_lookup  _ _ _ _ _ EQ) as [EQ1 [EQ2 EQ3]].
+  intros l1 stk1 Eq1.
+  case (decide (l1.1 = l.1)) => [Eql|NEql];
+    [case (decide (l.2 ≤ l1.2 < l.2 + n)) => [[Le Lt]|NIN]|].
+  - have Eql2: l1 = l +ₗ Z.of_nat (Z.to_nat (l1.2 - l.2)). {
+      destruct l, l1. move : Eql Le => /= -> ?.
+      rewrite /shift_loc /= Z2Nat.id; [|lia]. f_equal. lia. }
+    destruct (EQ1 (Z.to_nat (l1.2 - l.2)) stk1)
+      as [stk [Eq [[n1 stk'] [Eq' Eq0]]%bind_Some]];
+      [rewrite -(Nat2Z.id n) -Z2Nat.inj_lt; lia|by rewrite -Eql2|].
+    simpl in Eq0. simplify_eq. rewrite -Eql2 in Eq. naive_solver.
+  - rewrite EQ3; [naive_solver|].
+    intros i Lt Eq. apply NIN. rewrite Eq /=. lia.
+  - rewrite EQ3; [naive_solver|].
+    intros i Lt Eq. apply NEql. by rewrite Eq.
+Qed.
+
+(** Head preserving *)
+Definition is_stack_head (it: item) (stk: stack) :=
+  ∃ stk', stk = it :: stk'.
+
+Lemma sublist_head_preserving t it it' stk stk' :
+  stk' `sublist_of` stk →
+  it'.(tg) = Tagged t → it.(tg) = Tagged t →
+  it' ∈ stk' →
+  stack_item_tagged_NoDup stk →
+  is_stack_head it stk →
+  is_stack_head it stk'.
+Proof.
+  intros SUB Eqt' Eqt In' ND.
+  induction SUB as [|???? IH|???? IH]; [done|..]; intros [stk1 ?]; simplify_eq;
+    [by eexists|].
+  exfalso. move : ND.
+  rewrite /stack_item_tagged_NoDup filter_cons decide_True;
+    last by rewrite /is_tagged Eqt.
+  rewrite fmap_cons NoDup_cons. intros [NI ?].
+  apply NI, elem_of_list_fmap. exists it'. split; [rewrite Eqt' Eqt //|].
+  apply elem_of_list_filter. split. by rewrite /is_tagged Eqt'. by rewrite <-SUB.
+Qed.
+
+Lemma replace_check'_head_preserving stk stk' acc stk0 cids pm pm' t opro:
+  stack_item_tagged_NoDup (acc ++ stk ++ stk0) →
+  pm ≠ Disabled →
+  mkItem pm (Tagged t) opro ∈ (stk' ++ stk0) →
+  replace_check' cids acc stk = Some stk' →
+  is_stack_head (mkItem pm' (Tagged t) opro) (acc ++ stk ++ stk0) →
+  is_stack_head (mkItem pm' (Tagged t) opro) (stk' ++ stk0).
+Proof.
+  intros ND NDIS IN. revert acc ND.
+  induction stk as [|it stk IH]; simpl; intros acc ND.
+  { intros ?. by simplify_eq. }
+  case decide => ?; [case check_protector; [|done]|];
+    [|move => /IH; rewrite -(app_assoc acc [it] (stk ++ stk0)); naive_solver].
+  move => RC.
+  rewrite (app_assoc acc [it] (stk ++ stk0)).
+  have ND3: stack_item_tagged_NoDup
+    ((acc ++ [mkItem Disabled it.(tg) it.(protector)]) ++ stk ++ stk0).
+  { move : ND. clear.
+    rewrite (app_assoc acc [it]) 2!(Permutation_app_comm acc) -2!app_assoc.
+    rewrite /stack_item_tagged_NoDup 2!filter_cons /=.
+    case decide => ?; [rewrite decide_True //|rewrite decide_False //]. }
+  intros HD. apply (IH _ ND3 RC). clear IH. move : HD.
+  destruct acc as [|it1 acc]; last first.
+  { simpl in *. move => [? Eq]. inversion Eq. simplify_eq. by eexists. }
+  simpl. intros [stk2 Eq]. exfalso. simplify_eq; simpl in *.
+  have IN1:= (replace_check'_acc_result _ _ _ _ RC).
+  have IN': mkItem Disabled (Tagged t) opro ∈ stk' ++ stk0 by set_solver. clear IN1.
+  have ND4 := replace_check'_stack_item_tagged_NoDup_2 _ _ _ _ _ RC ND3.
+  have EQ := stack_item_tagged_NoDup_eq _ _ _ _ ND4 IN IN' eq_refl eq_refl.
+  by inversion EQ.
+Qed.
+
+Lemma replace_check_head_preserving stk stk' stk0 cids pm pm' t opro:
+  stack_item_tagged_NoDup (stk ++ stk0) →
+  pm ≠ Disabled →
+  mkItem pm (Tagged t) opro ∈ (stk' ++ stk0) →
+  replace_check cids stk = Some stk' →
+  is_stack_head (mkItem pm' (Tagged t) opro) (stk ++ stk0) →
+  is_stack_head (mkItem pm' (Tagged t) opro) (stk' ++ stk0).
+Proof. intros. eapply replace_check'_head_preserving; eauto. done. Qed.
+
+Lemma access1_head_preserving stk stk' kind tg cids n pm pm' t opro:
+  stack_item_tagged_NoDup stk →
+  pm ≠ Disabled →
+  mkItem pm (Tagged t) opro ∈ stk' →
+  access1 stk kind tg cids = Some (n, stk') →
+  is_stack_head (mkItem pm' (Tagged t) opro) stk →
+  is_stack_head (mkItem pm' (Tagged t) opro) stk'.
+Proof.
+  intros ND NDIS IN.
+  rewrite /access1. case find_granting as [gip|]; [|done]. simpl.
+  destruct kind.
+  - case replace_check as [stk1|] eqn:Eq; [|done].
+    simpl. intros ?. simplify_eq.
+    rewrite -{1}(take_drop gip.1 stk). intros HD.
+    rewrite -{1}(take_drop gip.1 stk) in ND.
+    eapply replace_check_head_preserving; eauto.
+  - case find_first_write_incompatible as [idx|]; [|done]. simpl.
+    case remove_check as [stk1|] eqn:Eq; [|done].
+    simpl. intros ?. simplify_eq.
+    have SUB: stk1 ++ drop gip.1 stk `sublist_of` stk.
+    { rewrite -{2}(take_drop gip.1 stk). apply sublist_app; [|done].
+      move : Eq. apply remove_check_sublist. }
+    eapply sublist_head_preserving; eauto. done.
+Qed.
+
+(** active_SRO preserving *)
+Lemma active_SRO_cons_elem_of t it stk :
+  t ∈ active_SRO (it :: stk) ↔
+  it.(perm) = SharedReadOnly ∧ (it.(tg) = Tagged t ∨ t ∈ active_SRO stk).
+Proof.
+  simpl. destruct it.(perm); [set_solver..| |set_solver].
+  case tg => [?|]; [rewrite elem_of_union elem_of_singleton|]; naive_solver.
+Qed.
+
+Lemma sublist_active_SRO_preserving t it stk stk' :
+  stk' `sublist_of` stk →
+  it.(tg) = Tagged t →
+  it ∈ stk' →
+  stack_item_tagged_NoDup stk →
+  t ∈ active_SRO stk → t ∈ active_SRO stk'.
+Proof.
+  intros SUB Eqt In' ND.
+  induction SUB as [|it1 stk1 stk2 ? IH|it1 stk1 stk2 ? IH]; [done|..].
+  - intros [? Eq]%active_SRO_cons_elem_of. apply active_SRO_cons_elem_of.
+    split; [done|]. destruct Eq as [?|Eq]; [by left|].
+    apply elem_of_cons in In' as [?|In'].
+    + subst it. rewrite Eqt. by left.
+    + right. apply IH; auto. by eapply stack_item_tagged_NoDup_cons_1.
+  - intros [? Eq]%active_SRO_cons_elem_of.
+    destruct Eq as [Eq|In2].
+    + exfalso. move : ND.
+      rewrite /stack_item_tagged_NoDup filter_cons decide_True;
+        last by rewrite /is_tagged Eq.
+      rewrite fmap_cons NoDup_cons. intros [NI ?].
+      apply NI, elem_of_list_fmap. exists it. split; [rewrite Eqt Eq //|].
+      apply elem_of_list_filter. split. by rewrite /is_tagged Eqt. by rewrite <-SUB.
+    + apply IH; auto. by eapply stack_item_tagged_NoDup_cons_1.
+Qed.
+
+Lemma active_SRO_tag_eq_elem_of stk1 stk2 t :
+  fmap tg stk1 = fmap tg stk2 →
+  Forall2 (λ pm1 pm2, pm1 = SharedReadOnly → pm2 = SharedReadOnly)
+          (fmap perm stk1) (fmap perm stk2) →
+  t ∈ active_SRO stk1 → t ∈ active_SRO stk2.
+Proof.
+  revert stk2.
+  induction stk1 as [|it stk1 IH]; intros stk2; [simpl; set_solver|].
+  destruct stk2 as [|it2 stk2]; [naive_solver|].
+  rewrite 4!fmap_cons. inversion 1 as [Eqt].
+  inversion 1 as [|???? Eq1 FA]; subst. rewrite 2!active_SRO_cons_elem_of.
+  intros [EqSRO Eq]. specialize (Eq1 EqSRO). split; [done|].
+  destruct Eq as [Eq|In1].
+  - rewrite -Eqt. by left.
+  - right. by apply IH.
+Qed.
+
+Lemma replace_check'_active_SRO_preserving cids acc stk stk' stk0 t it:
+  it.(tg) = Tagged t →
+  it ∈ stk' ++ stk0 →
+  replace_check' cids acc stk = Some stk' →
+  stack_item_tagged_NoDup (acc ++ stk ++ stk0) →
+  t ∈ active_SRO (acc ++ stk ++ stk0) → t ∈ active_SRO (stk' ++ stk0).
+Proof.
+  intros Eqt IN. revert acc.
+  induction stk as [|it1 stk IH]; simpl; intros acc.
+  { intros ?. by simplify_eq. }
+  case decide => [EqU|?]; [case check_protector; [|done]|];
+    [|move => /IH; rewrite -(app_assoc acc [it1] (stk ++ stk0)); naive_solver].
+  move => RC ND.
+  rewrite (app_assoc acc [it1] (stk ++ stk0)).
+  have ND3: stack_item_tagged_NoDup
+    ((acc ++ [mkItem Disabled it1.(tg) it1.(protector)]) ++ stk ++ stk0).
+  { move : ND. clear.
+    rewrite (app_assoc acc [it1]) 2!(Permutation_app_comm acc) -2!app_assoc.
+    rewrite /stack_item_tagged_NoDup 2!filter_cons /=.
+    case decide => ?; [rewrite decide_True //|rewrite decide_False //]. }
+  intros HD. apply (IH _ RC ND3). clear IH. move : HD.
+  apply active_SRO_tag_eq_elem_of.
+  - by rewrite !fmap_app /=.
+  - rewrite 2!(fmap_app _ _ (stk ++ stk0)).
+    apply Forall2_app; [rewrite 2!fmap_app; apply Forall2_app|].
+    + by apply Forall_Forall2_diag, Forall_forall.
+    + apply Forall2_cons; [|constructor]. by rewrite EqU.
+    + by apply Forall_Forall2_diag, Forall_forall.
+Qed.
+
+Lemma replace_check_active_SRO_preserving cids stk stk' stk0 it t:
+  it.(tg) = Tagged t →
+  it ∈ stk' ++ stk0 →
+  replace_check cids stk = Some stk' →
+  stack_item_tagged_NoDup (stk ++ stk0) →
+  t ∈ active_SRO (stk ++ stk0) → t ∈ active_SRO (stk' ++ stk0).
+Proof. by apply replace_check'_active_SRO_preserving. Qed.
+
+Lemma access1_active_SRO_preserving stk stk' kind tg cids n pm t opro:
+  stack_item_tagged_NoDup stk →
+  mkItem pm (Tagged t) opro ∈ stk' →
+  access1 stk kind tg cids = Some (n, stk') →
+  t ∈ active_SRO stk → t ∈ active_SRO stk'.
+Proof.
+  intros ND IN.
+  rewrite /access1. case find_granting as [gip|]; [|done]. simpl.
+  destruct kind.
+  - case replace_check as [stk1|] eqn:Eq; [|done].
+    simpl. intros ?. simplify_eq.
+    rewrite -{1}(take_drop gip.1 stk). intros HD.
+    rewrite -{1}(take_drop gip.1 stk) in ND.
+    eapply replace_check_active_SRO_preserving; eauto. done.
+  - case find_first_write_incompatible as [idx|]; [|done]. simpl.
+    case remove_check as [stk1|] eqn:Eq; [|done].
+    simpl. intros ?. simplify_eq.
+    have SUB: stk1 ++ drop gip.1 stk `sublist_of` stk.
+    { rewrite -{2}(take_drop gip.1 stk). apply sublist_app; [|done].
+      move : Eq. apply remove_check_sublist. }
+    eapply sublist_active_SRO_preserving; eauto. done.
+Qed.
+
+(** Removing incompatible items *)
+
+Lemma find_granting_incompatible_head stk kind t ti idx pm pmi oproi
+  (HD: is_stack_head (mkItem pmi (Tagged t) oproi) stk)
+  (NEQ: Tagged t ≠ ti) :
+  find_granting stk kind ti = Some (idx, pm) →
+  is_stack_head (mkItem pmi (Tagged t) oproi) (take idx stk).
+Proof.
+  destruct HD as [stk' Eqi]. rewrite Eqi.
+  rewrite /find_granting /= decide_False; last (intros [_ Eq]; by inversion Eq).
+  case list_find => [[idx' pm'] /=|//]. intros . simplify_eq. simpl.
+  by eexists.
+Qed.
+
+(* Writing *)
+Lemma find_first_write_incompatible_head stk pm idx t opro pmi
+  (HD: is_stack_head (mkItem pmi t opro) stk)
+  (NSRW: pmi ≠ SharedReadWrite) :
+  find_first_write_incompatible stk pm = Some idx → (0 < idx)%nat.
+Proof.
+  set it := (mkItem pmi t opro).
+  destruct HD as [stk' Eqi]. rewrite Eqi.
+  destruct pm; [..|done|done]; simpl.
+  - intros. simplify_eq. lia.
+  - rewrite reverse_cons.
+    destruct (list_find_elem_of (λ it, it.(perm) ≠ SharedReadWrite)
+                (reverse stk' ++ [it]) it) as [[id fnd] Eqf]; [set_solver|done|].
+    rewrite Eqf.
+    intros. simplify_eq. apply list_find_Some in Eqf as [Eqi ?].
+    apply lookup_lt_Some in Eqi.
+    rewrite app_length /= reverse_length Nat.add_1_r in Eqi. lia.
+Qed.
+
+Lemma remove_check_incompatible_items cids stk stk' stk0 n it i t
+  (ND: stack_item_tagged_NoDup (stk ++ stk0)) :
+  it.(tg) = Tagged t → stk !! i = Some it → (i < n)%nat →
+  remove_check cids stk n = Some stk' →
+  ∀ it', it'.(tg) = Tagged t → it' ∈ (stk' ++ stk0) → False.
+Proof.
+  intros Eqt. revert i stk stk0 ND.
+  induction n as [|n IH]; simpl; intros i stk stk0 ND Eqit Lt; [lia|].
+  destruct stk as [|it' stk]; [done|]. simpl.
+  case check_protector; [|done].
+  destruct i as [|i].
+  - simpl in Eqit. simplify_eq.
+    intros SUB%remove_check_sublist it' Eq' IN.
+    have SUB': stk' ++ stk0 `sublist_of` stk ++ stk0 by apply sublist_app.
+    rewrite -> SUB' in IN.
+    clear -ND Eqt Eq' IN.
+    move : ND.
+    rewrite /stack_item_tagged_NoDup filter_cons decide_True;
+            [|by rewrite /is_tagged Eqt].
+    rewrite fmap_cons NoDup_cons Eqt -Eq'.
+    intros [IN' _]. apply IN'. apply elem_of_list_fmap.
+    exists it'. split; [done|]. apply elem_of_list_filter. by rewrite /is_tagged Eq'.
+  - apply (IH i); [|done|lia]. by apply stack_item_tagged_NoDup_cons_1 in ND.
+Qed.
+
+Lemma access1_write_remove_incompatible_head stk t ti cids n stk'
+  (ND: stack_item_tagged_NoDup stk) :
+  (∃ oproi, is_stack_head (mkItem Unique (Tagged ti) oproi) stk) →
+  access1 stk AccessWrite t cids = Some (n, stk') →
+  Tagged ti ≠ t →
+  ∀ pm opro, (mkItem pm (Tagged ti) opro) ∈ stk' → False.
+Proof.
+  intros HD. rewrite /access1.
+  case find_granting as [[n' pm']|] eqn:GRANT; [|done]. simpl.
+  case find_first_write_incompatible as [idx|] eqn:INC; [|done]. simpl.
+  case remove_check as [stk1|] eqn:Eq; [|done].
+  simpl. intros ?. simplify_eq.
+  intros NEQ. destruct HD as [oproi HD].
+  have HD' := find_granting_incompatible_head _ _ _ _ _ _ _ _ HD NEQ GRANT.
+  have Gt0 := find_first_write_incompatible_head _ _ _ _ _ _ HD' (ltac:(done)) INC.
+  rewrite -{1}(take_drop n stk) in ND.
+  intros pm opro.
+  have EQH : take n stk !! 0%nat = Some (mkItem Unique (Tagged ti) oproi).
+  { destruct HD' as [? Eq']. by rewrite Eq'. }
+  eapply (remove_check_incompatible_items _ _ _ _ idx
+            (mkItem Unique (Tagged ti) oproi) O ti ND); done.
+Qed.
+
+(* Reading *)
+Lemma replace_check'_incompatible_items cids acc stk stk' stk0 it t
+  (ND: stack_item_tagged_NoDup (acc ++ stk ++ stk0)) :
+  it.(tg) = Tagged t → it.(perm) = Unique → it ∈ stk →
+  replace_check' cids acc stk = Some stk' →
+  ∀ it', it'.(tg) = Tagged t → it' ∈ (stk' ++ stk0) → it'.(perm) = Disabled.
+Proof.
+  intros Eqt IU IN. revert acc ND.
+  induction stk as [|it0 stk IH]; simpl; intros acc ND; [set_solver|].
+  case decide => ?; [case check_protector; [|done]|]; last first.
+  { move => /(IH ltac:(set_solver)).
+    rewrite -(app_assoc acc [it0] (stk ++ stk0)).
+    intros IH1 it' Eqit' Init'. apply IH1; [done..|]. clear -Init'. set_solver. }
+  move => RC.
+  have ND3: stack_item_tagged_NoDup
+    ((acc ++ [mkItem Disabled it0.(tg) it0.(protector)]) ++ stk ++ stk0).
+  { move : ND. clear.
+    rewrite (app_assoc acc [it0]) 2!(Permutation_app_comm acc) -2!app_assoc.
+    rewrite /stack_item_tagged_NoDup 2!filter_cons /=.
+    case decide => ?; [rewrite decide_True //|rewrite decide_False //]. }
+  have IN1:= (replace_check'_acc_result _ _ _ _ RC).
+  have IN': mkItem Disabled it0.(tg) it0.(protector) ∈ stk' ++ stk0 by set_solver.
+  have ND4 := replace_check'_stack_item_tagged_NoDup_2 _ _ _ _ _ RC ND3.
+  apply elem_of_cons in IN as [|IN].
+  { intros it' Eqt' Init'. subst it0.
+    have ? : it' = mkItem Disabled it.(tg) it.(protector).
+    { apply (stack_item_tagged_NoDup_eq _ _ _ t ND4 Init' IN' Eqt').
+      by rewrite Eqt. }
+    by subst it'. }
+  apply (IH IN _ ND3 RC).
+Qed.
+
+Lemma replace_check_incompatible_items cids stk stk' stk0 it t
+  (ND: stack_item_tagged_NoDup (stk ++ stk0)) :
+  it.(tg) = Tagged t → it.(perm) = Unique → it ∈ stk →
+  replace_check cids stk = Some stk' →
+  ∀ it', it'.(tg) = Tagged t → it' ∈ (stk' ++ stk0) → it'.(perm) = Disabled.
+Proof. intros ????. eapply (replace_check'_incompatible_items _ []); eauto. Qed.
+
+Lemma access1_read_replace_incompatible_head stk t ti cids n stk'
+  (ND: stack_item_tagged_NoDup stk) :
+  (∃ oproi, is_stack_head (mkItem Unique (Tagged ti) oproi) stk) →
+  access1 stk AccessRead t cids = Some (n, stk') →
+  Tagged ti ≠ t →
+  ∀ pm opro, (mkItem pm (Tagged ti) opro) ∈ stk' → pm = Disabled.
+Proof.
+  intros HD. rewrite /access1.
+  case find_granting as [[n' pm']|] eqn:GRANT; [|done]. simpl.
+  case replace_check as [stk1|] eqn:Eq; [|done].
+  simpl. intros ?. simplify_eq.
+  intros NEQ pm opro. destruct HD as [oproi HD].
+  rewrite -{1}(take_drop n stk) in ND.
+  eapply (replace_check_incompatible_items _ _ _ _ (mkItem Unique (Tagged ti) oproi) ti ND);
+    try done.
+  have HD' := find_granting_incompatible_head _ _ _ _ _ _ _ _ HD NEQ GRANT.
+  clear -HD'. destruct HD' as [? EqD]. rewrite EqD. by left.
+Qed.
+
+Lemma active_SRO_elem_of t stk :
+  t ∈ active_SRO stk → ∃ i it, stk !! i = Some it ∧ it.(tg) = Tagged t ∧
+  it.(perm) = SharedReadOnly ∧
+  ∀ j jt, (j < i)%nat → stk !! j = Some jt → jt.(perm) = SharedReadOnly.
+Proof.
+  induction stk as [|it' stk IH]; simpl; [set_solver|].
+  destruct it'.(perm) eqn:Eqp; [set_solver..| |set_solver].
+  destruct it'.(tg) eqn:Eqt;
+    [rewrite elem_of_union elem_of_singleton; intros [?|Eq]; [subst|]|].
+  - exists O, it'. repeat split; [done..|intros; lia].
+  - destruct (IH Eq) as (i & it1 & ? & ? & ? & HL).
+    exists (S i), it1. repeat split; [done..|].
+    intros j jt Lt. destruct j; simpl.
+    + intros. by simplify_eq.
+    + apply HL. lia.
+  - intros Eq. destruct (IH Eq) as (i & it1 & ? & ? & ? & HL).
+    exists (S i), it1. repeat split; [done..|].
+    intros j jt Lt. destruct j; simpl.
+    + intros. by simplify_eq.
+    + apply HL. lia.
+Qed.
+
+Lemma active_SRO_elem_of_inv i it t stk :
+  stk !! i = Some it → it.(tg) = Tagged t →
+  it.(perm) = SharedReadOnly →
+  (∀ j jt, (j < i)%nat → stk !! j = Some jt → jt.(perm) = SharedReadOnly) →
+  t ∈ active_SRO stk.
+Proof.
+  revert i.
+  induction stk as [|it' stk IH]; [set_solver|].
+  intros [|i]; intros Eq; simpl in Eq.
+  { simplify_eq. intros. apply active_SRO_cons_elem_of. split; [done|by left]. }
+  intros Eqt SRO PREV.
+  apply active_SRO_cons_elem_of.
+  have SRO' := PREV O it' ltac:(lia) eq_refl. split; [done|].
+  right. apply (IH _ Eq Eqt SRO).
+  intros j jt Lt. apply (PREV (S j) jt). lia.
+Qed.
+
+Lemma find_granting_incompatible_active_SRO stk t ti idx pm
+  (HD: ti ∈ active_SRO stk) :
+  find_granting stk AccessWrite t = Some (idx, pm) →
+  ti ∈ active_SRO (take idx stk).
+Proof.
+  revert idx. induction stk as [|it stk IH]; simpl; intros idx; [set_solver|].
+  move : HD. rewrite /find_granting /=.
+  destruct it.(perm) eqn:Eqp; [set_solver..| |set_solver].
+  rewrite decide_False; last (intros [PM _]; by rewrite Eqp in PM).
+  destruct (list_find (matched_grant AccessWrite t) stk)
+    as [[n' pm']|] eqn:Eql; [|done].
+  simpl. intros IN ?. simplify_eq. rewrite /= Eqp. move : IN.
+  destruct it.(tg) eqn:Eqt; simpl;
+    [rewrite elem_of_union elem_of_singleton; intros [|IN]; [subst|]|]; simpl.
+  - set_solver.
+  - rewrite elem_of_union. right. apply IH. done. by rewrite /find_granting Eql.
+  - intros ?. apply IH. done. by rewrite /find_granting Eql.
+Qed.
+
+Lemma find_first_write_incompatible_active_SRO stk pm idx :
+  find_first_write_incompatible stk pm = Some idx →
+  ∀ t, t ∈ active_SRO stk → ∃ i it, stk !! i = Some it ∧
+    it.(perm) = SharedReadOnly ∧
+    it.(tg) = Tagged t ∧ (i < idx)%nat ∧
+    (∀ (j : nat) (jt : item), (j < i)%nat → stk !! j = Some jt →
+        jt.(perm) = SharedReadOnly).
+Proof.
+  intros EF t IN.
+  destruct (active_SRO_elem_of _ _ IN) as (i1 & it1 & Eqit1 & Eqt1 & Eqp1 & HL1).
+  move  : EF.
+  destruct pm; [| |done..].
+  { simpl. intros. simplify_eq. exists i1, it1.
+    repeat split; [done..| |done]. by eapply lookup_lt_Some. }
+  simpl.
+  destruct (list_find_elem_of (λ it, it.(perm) ≠ SharedReadWrite) (reverse stk) it1)
+    as [[n1 pm1] Eqpm1].
+  { rewrite elem_of_reverse. by eapply elem_of_list_lookup_2. }
+  { by rewrite Eqp1. }
+  rewrite Eqpm1. intros. simplify_eq.
+  exists i1, it1. repeat split; [done..| |done].
+  apply list_find_Some_not_earlier in Eqpm1 as (Eqrv & Eqpmv & HLv).
+  case (decide (i1 + n1 < length stk)%nat) => [?|]; [lia|].
+  rewrite Nat.nlt_ge => GE. exfalso.
+  destruct (reserve_lookup _ _ _ Eqit1) as (j & Eqj & Eql).
+  have Lt: (j < n1)%nat by lia.
+  specialize (HLv _ _ Lt Eqj). rewrite Eqp1 in HLv. by apply HLv.
+Qed.
+
+Lemma access1_write_remove_incompatible_active_SRO stk t ti cids n stk'
+  (ND: stack_item_tagged_NoDup stk) :
+  (ti ∈ active_SRO stk) →
+  access1 stk AccessWrite t cids = Some (n, stk') →
+  ∀ pm opro, (mkItem pm (Tagged ti) opro) ∈ stk' → False.
+Proof.
+  intros HD. rewrite /access1.
+  case find_granting as [[n' pm']|] eqn:GRANT; [|done]. simpl.
+  case find_first_write_incompatible as [idx|] eqn:INC; [|done]. simpl.
+  case remove_check as [stk1|] eqn:Eq; [|done].
+  simpl. intros ?. simplify_eq.
+  intros NEQ.
+  have HD' := find_granting_incompatible_active_SRO _ _ _ _ _ HD GRANT.
+  destruct (find_first_write_incompatible_active_SRO _ _ _ INC _ HD')
+    as (i & it & Eqi & Eqp & Eqt & Lt & HL).
+  rewrite -{1}(take_drop n stk) in ND. intros ?.
+  eapply (remove_check_incompatible_items _ _ _ _ idx it i ti ND); eauto.
+Qed.
+
+Lemma access1_incompatible_head_protector stk t ti kind cids n stk' c :
+  (is_stack_head (mkItem Unique (Tagged t) (Some c)) stk) →
+  c ∈ cids →
+  access1 stk kind ti cids = Some (n, stk') →
+  ti = Tagged t.
+Proof.
+  intros HD ACTIVE. case (decide (Tagged t = ti)) => NEQ; [done|].
+  rewrite /access1.
+  case find_granting as [[n' pm']|] eqn:GRANT; [|done]. simpl.
+  destruct kind.
+  - case replace_check as [stk1|] eqn:Eq; [|done].
+    simpl. intros ?. simplify_eq.
+    have HD' := find_granting_incompatible_head _ _ _ _ _ _ _ _ HD NEQ GRANT.
+    destruct HD' as [stk' Eqs].
+    move : Eq.
+    rewrite Eqs /replace_check /= /check_protector /= /is_active bool_decide_true //.
+  - have HD' := find_granting_incompatible_head _ _ _ _ _ _ _ _ HD NEQ GRANT.
+    case find_first_write_incompatible as [idx|] eqn:INC; [|done]. simpl.
+    have NONEZ: (0 < idx)%nat.
+    { eapply (find_first_write_incompatible_head _ _ _ _ _ _ HD'); eauto. }
+    destruct HD' as [stk2 Eqs].
+    rewrite Eqs /=. destruct idx; [lia|].
+    rewrite /= /check_protector /= /is_active bool_decide_true //.
+Qed.
+
+
+Lemma tag_unique_head_access cids stk t opro kind :
+  is_stack_head (mkItem Unique t opro) stk →
+  ∃ n, access1 stk kind t cids = Some (n, stk).
+Proof.
+  intros [stk1 Eqstk].
+  rewrite /access1.
+  have Eq1: list_find (matched_grant kind t) stk =
+    Some (O, mkItem Unique t opro).
+  { apply list_find_Some_not_earlier. split; last split.
+    rewrite Eqstk //. done. intros; lia. }
+  have Eq2: find_granting stk kind t = Some (O, Unique).
+  { rewrite /= /find_granting Eq1 //. }
+  rewrite Eq2 /=.
+  exists O. by destruct kind.
+Qed.
+
+Lemma replace_check'_preserve cids acc stk :
+  (∀ it, it ∈ stk → it.(perm) ≠ Unique) →
+  replace_check' cids acc stk = Some (acc ++ stk).
+Proof.
+  revert acc. induction stk as [|it' stk IH]; intros acc IN.
+  { rewrite /= app_nil_r //. }
+  rewrite /= decide_False; last by (apply IN; left).
+  rewrite (app_assoc acc [it'] stk). apply IH. set_solver.
+Qed.
+
+Lemma replace_check_preserve cids stk :
+  (∀ it, it ∈ stk → it.(perm) ≠ Unique) →
+  replace_check cids stk = Some stk.
+Proof. apply replace_check'_preserve. Qed.
+
+Lemma tag_SRO_top_access cids stk t :
+  t ∈ active_SRO stk →
+  ∃ n, access1 stk AccessRead (Tagged t) cids = Some (n, stk).
+Proof.
+  intros IN.
+  destruct (active_SRO_elem_of _ _ IN) as (i1 & it1 & Eqit1 & Eqt1 & Eqp1 & HL1).
+  rewrite /= /access1.
+   have Eq1: is_Some (list_find (matched_grant AccessRead (Tagged t)) stk).
+  { apply (list_find_elem_of _ _ it1).
+    by eapply elem_of_list_lookup_2. by rewrite /matched_grant Eqp1. }
+  destruct Eq1 as [[n2 it2] Eq2].
+  have Eq3: find_granting stk AccessRead (Tagged t) = Some (n2, it2.(perm)).
+  { rewrite /= /find_granting Eq2 //. }
+  rewrite Eq3 /=. exists n2.
+  rewrite replace_check_preserve.
+  - rewrite /= take_drop //.
+  - apply list_find_Some_not_earlier in Eq2 as (Eq2 & GR & LT).
+    have Lti1: (n2 ≤ i1)%nat.
+    { case (decide (n2 ≤ i1)%nat) => [//|/Nat.nle_gt Lt].
+      exfalso. apply (LT _ _ Lt Eqit1). rewrite /matched_grant Eqp1 //. }
+    intros it [k Eqk]%elem_of_list_lookup_1.
+    have Ltk : (k < n2)%nat.
+    { rewrite -(take_length_le stk n2).
+      by eapply lookup_lt_Some. apply Nat.lt_le_incl; by eapply lookup_lt_Some. }
+    have HL: stk !! k = Some it. { rewrite -(lookup_take _ n2) //. }
+    have Ltk2: (k < i1)%nat. { eapply Nat.lt_le_trans; eauto. }
+    by rewrite (HL1 _ _ Ltk2 HL).
+Qed.
+
+(** Tag-on-top *)
+Lemma tag_on_top_write σ l tg stks :
+  tag_on_top σ.(sst) l tg Unique →
+  memory_written (sst σ) (scs σ) l (Tagged tg) 1 = Some stks →
+  tag_on_top stks l tg Unique.
+Proof.
+  rewrite /memory_written /tag_on_top /= shift_loc_0.
+  destruct (sst σ !! l) eqn:Hlk; last done. simpl.
+  destruct s as [|it st]; first done. simpl.
+  destruct it as [perm tg' prot']. intros [prot ?]; simplify_eq/=.
+  edestruct tag_unique_head_access as [n ->].
+  { eexists. done. }
+  simpl. intros. simplify_eq/=. eexists. rewrite lookup_insert.
+  simpl. done.
+Qed.
+
+Lemma tag_on_top_grant_uniq_SRO stk old it cids  stk'
+  (UNIQ: it.(perm) = Unique ∨ it.(perm) = SharedReadOnly) :
+  grant stk old it cids = Some stk' → is_stack_head it stk'.
+Proof.
+  rewrite /grant.
+  case find_granting as [gip|]; [|done].
+  destruct UNIQ as [UNIQ|UNIQ];
+  rewrite /= UNIQ /=; (case access1 => [[n1 stk1]/=|//]);
+  (destruct stk1; [|case decide => ?]; intros; simplify_eq; by eexists).
+Qed.
+
+Lemma tag_on_top_reborrowN_uniq_SRO α cids l n to tn pm α' pro
+  (UNIQ: pm = Unique ∨ pm = SharedReadOnly) :
+  reborrowN α cids l n to (Tagged tn) pm pro = Some α' →
+  ∀ i, (i < n)%nat → tag_on_top α' (l +ₗ i) tn pm.
+Proof.
+  intros RB i Lt.
+  destruct (for_each_lookup_case_2 _ _ _ _ _ RB) as [EQ _].
+  specialize (EQ _ Lt) as (stk & stk' & Eq & Eq' & GR).
+  apply tag_on_top_grant_uniq_SRO in GR as [stk1 Eq1]; [|done].
+  rewrite /tag_on_top Eq' Eq1 /=. by eexists.
+Qed.
+
+Lemma tag_on_top_retag_ref_uniq α cids nxtp l old T pro tn α' nxtp' :
+  retag_ref α cids nxtp l old T (UniqueRef false) pro
+    = Some (Tagged tn, α', nxtp') →
+  ∀ i, (i < tsize T)%nat → tag_on_top α' (l +ₗ i) tn Unique.
+Proof.
+  intros RT i. destruct (tsize T) as [|n] eqn:Eqsz; [lia|].
+  rewrite -Eqsz.
+  move : RT. rewrite /retag_ref {1}Eqsz /=.
+  case reborrowN as [α1|] eqn:RB; [|done]. simpl. intros ?. simplify_eq.
+  eapply tag_on_top_reborrowN_uniq_SRO; eauto.
+Qed.
+
+Lemma tag_on_top_retag_ref_shr α cids nxtp l old T pro tn α' nxtp'
+  (FRZ: is_freeze T) :
+  retag_ref α cids nxtp l old T SharedRef pro
+    = Some (Tagged tn, α', nxtp') →
+  ∀ i, (i < tsize T)%nat → tag_on_top α' (l +ₗ i) tn SharedReadOnly.
+Proof.
+  intros RT i. destruct (tsize T) as [|n] eqn:Eqsz; [lia|].
+  rewrite -Eqsz.
+  move : RT. rewrite /retag_ref {1}Eqsz /= visit_freeze_sensitive_is_freeze //.
+  case reborrowN as [α1|] eqn:RB; [|done]. simpl. intros ?. simplify_eq.
+  eapply tag_on_top_reborrowN_uniq_SRO; eauto.
+Qed.
+
+Lemma tag_on_top_shr_active_SRO α l t :
+  tag_on_top α l t SharedReadOnly →
+  ∃ stk, α !! l = Some stk ∧ t ∈ active_SRO stk.
+Proof.
+  intros [pro Eq]. destruct (α !! l) as [stk|]; [|done].
+  simpl in Eq. destruct stk as [|it stk']; [done|].
+  simpl in Eq. simplify_eq. eexists. split; [done|].
+  rewrite /= elem_of_union elem_of_singleton. by left.
+Qed.
+
+(* retag *)
+Lemma retag_nxtp_change α cids c nxtp l otag ntag rk pk T α' nxtp'
+  (TS: (O < tsize T)%nat)
+  (RK: match pk with | RawPtr _ => rk = RawRt | _ => True end) :
+  retag α nxtp cids c l otag rk pk T = Some (ntag, α', nxtp') →
+  nxtp' = S nxtp ∧
+  match ntag with
+  | Untagged => True
+  | Tagged t => nxtp = t
+  end.
+Proof.
+  assert (∃ n, tsize T = S n) as [n EqT].
+  { destruct (tsize T); [lia|by eexists]. }
+  destruct pk as [[]| |]; [| |subst rk|]; rewrite /retag /= /retag_ref EqT;
+  (case reborrow as [α1|]; [|done]); simpl; intros; by simplify_eq.
+Qed.
+
+Lemma retag_change_case α cids c nxtp l otag ntag rk pk T α' nxtp' :
+  retag α nxtp cids c l otag rk pk T = Some (ntag, α', nxtp') →
+  tsize T = O ∧ α' = α ∧ nxtp' = nxtp ∧ ntag = otag ∨
+  (O < tsize T)%nat ∧
+    match pk, rk with
+    | RawPtr _, RawRt => True
+    | RawPtr _, _ => α' = α ∧ nxtp' = nxtp ∧ ntag = otag
+    | _, _ => True
+    end.
+Proof.
+  destruct (tsize T) as [|n] eqn:EqT.
+  - rewrite /retag /retag_ref EqT /=.
+    destruct pk as [[]| |]; [| |destruct rk|]; simpl; intros; simplify_eq;
+      by left.
+  - rewrite /retag /retag_ref EqT /=.
+    destruct pk as [[]| |]; [| |destruct rk|]; simpl; intros; simplify_eq;
+      right; (split; [lia|done]).
+Qed.
+
+Lemma retag_change_tag α cids c nxtp l otag ntag rk pk T α' nxtp' :
+  retag α nxtp cids c l otag rk pk T = Some (ntag, α', nxtp') →
+  ntag = otag ∨
+  match ntag with
+  | Tagged t => t = nxtp ∧ nxtp' = S nxtp
+  | _ => True
+  end.
+Proof.
+  intros RT.
+  destruct (retag_change_case _ _ _ _ _ _ _ _ _ _ _ _ RT) as [[?[?[??]]]|[? Eq]].
+  - simplify_eq; by left.
+  - destruct pk.
+    + apply retag_nxtp_change in RT as []; [|done..]. right. by destruct ntag.
+    + destruct rk.
+      * left. by destruct Eq as [_ []]; subst.
+      * left. by destruct Eq as [_ []]; subst.
+      * apply retag_nxtp_change in RT as []; [|done..]. right. by destruct ntag.
+      * left. by destruct Eq as [_ []]; subst.
+    + apply retag_nxtp_change in RT as []; [|done..]. right. by destruct ntag.
+Qed.
+
+Lemma retag_change_nxtp α cids c nxtp l otag ntag rk pk T α' nxtp' :
+  retag α nxtp cids c l otag rk pk T = Some (ntag, α', nxtp') →
+  (nxtp ≤ nxtp')%nat.
+Proof.
+  intros RT.
+  destruct (retag_change_case _ _ _ _ _ _ _ _ _ _ _ _ RT) as [[?[?[??]]]|[? Eq]].
+  - by simplify_eq.
+  - destruct pk.
+    + apply retag_nxtp_change in RT as []; [lia|done..].
+    + destruct rk.
+      * by destruct Eq as [_ [? _]]; subst.
+      * by destruct Eq as [_ [? _]]; subst.
+      * apply retag_nxtp_change in RT as []; [lia|done..].
+      * by destruct Eq as [_ [? _]]; subst.
+    + apply retag_nxtp_change in RT as []; [lia|done..].
+Qed.
+
+Lemma retag_change_ref_NZST α nxtp cids c l otag rk mut T ntag α' nxtp':
+  (O < tsize T)%nat  →
+  retag α nxtp cids c l otag rk (RefPtr mut) T = Some (ntag, α', nxtp') →
+  ntag = Tagged nxtp ∧ nxtp' = S nxtp.
+Proof.
+  intros ST.
+  assert (∃ n, tsize T = S n) as [n EqT].
+  { destruct (tsize T); [lia|by eexists]. }
+  destruct mut; rewrite /retag /= /retag_ref EqT;
+  (case reborrow as [α1|]; [|done]); simpl; intros; by simplify_eq.
+Qed.
+
+Lemma unsafe_action_stacks_changed
+  (f: stacks → _ → nat → _ → _) α l (last fsz usz: nat) α' ln cn
+  (P: option stack → option stack → bool → Prop)
+  (HF: ∀ α1 α2 l n b, f α1 l n b = Some α2 →
+      (∀ l', (∀ (i : nat), (i < n)%nat → l' ≠ l +ₗ i) → α2 !! l' = α1 !! l') ∧
+      (∀ (i : nat), (i < n)%nat → P (α1 !! (l +ₗ i)) (α2 !! (l +ₗ i)) b)):
+  unsafe_action f α l last fsz usz = Some (α', (ln, cn)) →
+  (last ≤ ln)%nat ∧
+  (∀ l', (∀ (i : nat), (last ≤ i < ln)%nat → l' ≠ l +ₗ i) → α' !! l' = α !! l') ∧
+  (∀ (i : nat), (last ≤ i < ln)%nat → ∃ b, P (α !! (l +ₗ i)) (α' !! (l +ₗ i)) b).
+Proof.
+  rewrite /unsafe_action.
+  case f as [α1|] eqn:Eqf1; [simpl|done]. case (f α1) eqn:Eqf2; [simpl|done].
+  intros ?. simplify_eq. split; [lia|].
+  destruct (HF _ _ _ _ _ Eqf1) as [HF1 Eq1].
+  destruct (HF _ _ _ _ _ Eqf2) as [HF2 Eq2]. split.
+  { intros ? NEQ. rewrite HF2; last first.
+    - intros i Lt.
+      rewrite shift_loc_assoc -Nat2Z.inj_add. apply NEQ. lia.
+    - rewrite HF1 //.
+      intros ??. rewrite shift_loc_assoc -Nat2Z.inj_add. apply NEQ. lia. }
+  intros i [Le Lt].
+  case (decide (i < last + fsz)%nat) => [Lt1|Ge1].
+  - have Le1: (i - last < fsz)%nat by lia.
+    have Eql: l +ₗ i = l +ₗ last +ₗ (i - last)%nat.
+    { rewrite shift_loc_assoc. f_equal. lia. }
+    specialize (Eq1 _ Le1). rewrite -Eql in Eq1. rewrite HF2.
+    + by exists true.
+    + intros j Ltj.
+      rewrite shift_loc_assoc -Nat2Z.inj_add.
+      intros ?%shift_loc_inj%Z_of_nat_inj. subst i. lia.
+  - apply Nat.nlt_ge in Ge1.
+    have Le1: (i - (last + fsz) < usz)%nat by lia.
+    have Eql: l +ₗ i = l +ₗ (last + fsz)%nat +ₗ (i - (last + fsz))%nat.
+    { rewrite shift_loc_assoc. f_equal. lia. }
+    specialize (Eq2 _ Le1). rewrite -Eql in Eq2. rewrite -HF1.
+    + by exists false.
+    + intros ??. rewrite shift_loc_assoc -Nat2Z.inj_add.
+      intros ?%shift_loc_inj%Z_of_nat_inj. subst i. lia.
+Qed.
+
+
+Lemma visit_freeze_sensitive'_stacks_changed l (f: stacks → _ → _ → _ → _)
+  α α' last cur T l' c'
+  (P: option stack → option stack → bool → Prop) :
+  let HF (f: stacks → loc → nat → bool → option stacks) :=
+    ∀ α1 α2 l n b, f α1 l n b = Some α2 →
+      (∀ l', (∀ (i : nat), (i < n)%nat → l' ≠ l +ₗ i) → α2 !! l' = α1 !! l') ∧
+      (∀ (i : nat), (i < n)%nat → P (α1 !! (l +ₗ i)) (α2 !! (l +ₗ i)) b) in
+  let UC α1 α2 (l: loc) (lo ln: nat) :=
+    (lo ≤ ln)%nat ∧
+    (∀ l', (∀ (i : nat), (lo ≤ i < ln)%nat → l' ≠ l +ₗ i) → α2 !! l' = α1 !! l') ∧
+    (∀ (i : nat), (lo ≤ i < ln)%nat → ∃ b, P (α1 !! (l +ₗ i)) (α2 !! (l +ₗ i)) b) in
+  HF f →
+  visit_freeze_sensitive' l f α last cur T = Some (α', (l', c')) →
+  UC α α' l last l'.
+Proof.
+  intros HF UC.
+  apply (visit_freeze_sensitive'_elim
+    (* general goal P *)
+    (λ l f α l1 c1 T oalc, ∀ α' l' c',
+      HF f → oalc = Some (α', (l', c')) → UC α α' l l1 l')
+    (λ l f _ _ _ Ts1 α l1 c1 Ts2 oalc, ∀ α' l' c',
+      HF f → oalc = Some (α', (l', c')) →
+          UC α α' l l1 l')); rewrite /HF /UC.
+  - clear. intros l f α1 l1 c1 s1 α2 l2 c2 HF ?.
+    simplify_eq. split; [done|].
+    split; [naive_solver|]. clear. intros i []. lia.
+  - clear. intros l f α1 l1 c1 ?? α2 l2 c2 HF ?.
+    simplify_eq. split; [done|].
+    split; [naive_solver|]. clear. intros i []. lia.
+  - (* Unsafe case *)
+    clear. intros ?? α l1 c1 ? α2 l2 c2 HF.
+    eapply unsafe_action_stacks_changed; eauto.
+  - (* Union case *)
+    clear. intros ????????? HF0. case is_freeze.
+    + intros. simplify_eq. do 2 (split; [done|]).
+      clear. intros ? []. lia.
+    + intros UN. eapply unsafe_action_stacks_changed; eauto.
+  - clear. intros ?????? IH ??? HF. case is_freeze.
+    + intros. simplify_eq. do 2 (split; [done|]).
+      clear. intros ? []. lia.
+    + intros VS. eapply (IH _ _ _ HF); eauto.
+  - (* Sum case *)
+    clear. intros ????????? HF. case is_freeze.
+    + intros. simplify_eq. do 2 (split; [done|]).
+      clear. intros ? []. lia.
+    + intros UN. eapply unsafe_action_stacks_changed; eauto.
+  - clear. intros l f α1 l1 c1 Ts1 α2 l2 c2 α3 l3 c3 HF ?.
+    simplify_eq. split; [done|].
+    split; [naive_solver|]. clear. intros i []. lia.
+  - (* Product case *)
+    clear. intros l f α0 l0 c0 Ts1 α2 l2 c2 T Ts2 IH1 IH2 α3 l3 c3 HF.
+    case visit_freeze_sensitive' as [alc|] eqn:Eqa; [|done].
+    intros VS. destruct alc as [α1 [l1 c1]]. simpl in VS.
+    destruct (IH2 α1 l1 c1 HF eq_refl) as [Le2 [IH21 IH22]].
+    simpl in IH21, IH22.
+    destruct (IH1 (α1, (l1,c1)) α3 l3 c3) as [Le1 [IH11 IH12]];
+      [done..|simpl in Le1; split]; [lia|].
+    simpl in IH11, IH12.
+    split.
+    + intros ? NC. rewrite IH11; [rewrite IH21 //|].
+      * intros ??. apply NC. lia.
+      * intros ??. apply NC. lia.
+    + intros i [Le Lt].
+      case (decide (l1 ≤ i)%nat) => [Gel1|Ltl1].
+      * rewrite -IH21; [by apply IH12|].
+        intros j [Lej Ltj] ?%shift_loc_inj%Z_of_nat_inj. subst j. lia.
+      * apply Nat.nle_gt in Ltl1.
+        rewrite IH11; [by apply IH22|].
+        intros j [Lej Ltj] ?%shift_loc_inj%Z_of_nat_inj. subst j. lia.
+Qed.
+
+Lemma visit_freeze_sensitive_stacks_unchanged l
+  (f: stacks → _ → _ → _ → _)
+  α α' T
+  (P: option stack → option stack → bool → Prop) :
+  (∀ α1 α2 l n b, f α1 l n b = Some α2 →
+      (∀ l', (∀ (i : nat), (i < n)%nat → l' ≠ l +ₗ i) → α2 !! l' = α1 !! l') ∧
+      (∀ (i : nat), (i < n)%nat → P (α1 !! (l +ₗ i)) (α2 !! (l +ₗ i)) b)) →
+  visit_freeze_sensitive l T f α = Some α' →
+  (∀ l', (∀ (i : nat), (i < tsize T)%nat → l' ≠ l +ₗ i) → α' !! l' = α !! l') ∧
+  (∀ (i : nat), (i < tsize T)%nat → ∃ b, P (α !! (l +ₗ i)) (α' !! (l +ₗ i)) b).
+Proof.
+  intros HF.
+  rewrite /visit_freeze_sensitive.
+  case visit_freeze_sensitive' as [[α1 [l1 c1]]|] eqn:Eq; [|done].
+  intros Eqf.
+  have Eq' := Eq.
+  apply visit_freeze_sensitive'_offsets in Eq' as [_ Eq'].
+  rewrite 2!Nat.add_0_l in Eq'.
+  eapply visit_freeze_sensitive'_stacks_changed in Eq as [_ [EQ1 EQ2]]; [|done].
+  specialize (HF _ _ _ _ _ Eqf) as [HF1 HF2].
+  split.
+  - intros l' NEq. rewrite HF1; last first.
+    { intros i Lt. rewrite shift_loc_assoc -Nat2Z.inj_add.
+      apply NEq. rewrite -Eq'. lia. }
+    rewrite EQ1 //.
+    intros i [_ Lti]. apply NEq. rewrite -Eq'. lia.
+  - intros i Lt. rewrite -Eq' in Lt.
+    case (decide (i < l1)%nat) => [Ltl1|Gel1].
+    + rewrite HF1.
+      * apply EQ2. split; [lia|done].
+      * intros j Ltj. rewrite shift_loc_assoc_nat.
+        intros ?%shift_loc_inj%Z_of_nat_inj. subst i. lia.
+    + apply Nat.nlt_ge in Gel1. rewrite -EQ1.
+      * have Ltc1: (i - l1 < c1)%nat by lia.
+        specialize (HF2 _ Ltc1).
+        have Eql: l +ₗ l1 +ₗ (i - l1)%nat = l +ₗ i.
+        { rewrite shift_loc_assoc_nat. f_equal. lia. }
+        rewrite Eql in HF2. by exists true.
+      * intros j [_ Ltj] ?%shift_loc_inj%Z_of_nat_inj. subst i. lia.
+Qed.
+
+Lemma reborrowN_lookup_case (α1 α2 : stacks) cids l n old new pm protector
+  (EQB : reborrowN α1 cids l n old new pm protector = Some α2) :
+  (∀ l', (∀ (i : nat), (i < n)%nat → l' ≠ l +ₗ i) → α2 !! l' = α1 !! l') ∧
+  (∀ i, (i < n)%nat → ∃ stk stk',
+    α1 !! (l +ₗ i) = Some stk ∧
+    α2 !! (l +ₗ i) = Some stk' ∧
+    let item := mkItem pm new protector in
+    grant stk old item cids = Some stk').
+Proof.
+  destruct (for_each_lookup_case_2 _ _ _ _ _ EQB) as [HL1 HL2].
+  split; [done|].
+  intros i Lt. destruct (HL1 _ Lt) as (stk & stk' & Eq1 & Eq2 & GR).
+  naive_solver.
+Qed.
+
+Lemma reborrowN_visit_freeze_sensitive_case α α' l T cids old new protector :
+  let permB (b: bool) := if b then SharedReadOnly else SharedReadWrite in
+  let item (b: bool) := mkItem (permB b) new protector in
+  visit_freeze_sensitive l T
+        (λ α' l' sz frozen,
+          (* If is in Unsafe, use SharedReadWrite, otherwise SharedReadOnly *)
+          reborrowN α' cids l' sz old new (permB frozen) protector) α = Some α' →
+  (∀ l', (∀ (i : nat), (i < tsize T)%nat → l' ≠ l +ₗ i) → α' !! l' = α !! l') ∧
+  (∀ i, (i < tsize T)%nat → ∃ stk stk',
+    α !! (l +ₗ i) = Some stk ∧
+    α' !! (l +ₗ i) = Some stk' ∧ ∃ b,
+    grant stk old (item b) cids = Some stk').
+Proof.
+  intros permB item VS.
+  set P: option stack → option stack → bool → Prop :=
+    λ ostk ostk' b, ∃ stk stk', ostk = Some stk ∧ ostk' = Some stk' ∧
+      grant stk old (item b) cids = Some stk'.
+  apply (visit_freeze_sensitive_stacks_unchanged _ _ _ _ _ P) in VS.
+  - destruct VS as [VS1 VS2]. split; [done|].
+    intros i Lt. destruct (VS2 _ Lt) as (b & stk & stk' & Eq1 & Eq2 & Eq3).
+    naive_solver.
+  - clear. intros α1 α2 l n b [RB1 RB2]%reborrowN_lookup_case.
+    split; [done|]. intros i Lt.
+    specialize (RB2 _ Lt) as (stk & stk' & Eq1 & Eq2 & Eq3).
+    rewrite Eq1 Eq2. exists stk, stk'. naive_solver.
+Qed.
+
+Lemma reborrow_Some α α' cids l old T rk new protector :
+  reborrow α cids l old T rk new protector = Some α' →
+  (∀ l', (∀ (i : nat), (i < tsize T)%nat → l' ≠ l +ₗ i) → α' !! l' = α !! l') ∧
+  (∀ i, (i < tsize T)%nat → ∃ stk stk',
+    α !! (l +ₗ i) = Some stk ∧
+    α' !! (l +ₗ i) = Some stk' ∧
+    match rk with
+    | SharedRef | RawRef false =>
+      ∃ b : bool, grant stk old
+                 (mkItem (if b then SharedReadOnly else SharedReadWrite)
+                          new protector) cids = Some stk'
+    | UniqueRef false =>
+      grant stk old (mkItem Unique new protector) cids = Some stk'
+    | UniqueRef true | RawRef true =>
+      grant stk old (mkItem SharedReadWrite new protector) cids = Some stk'
+    end).
+Proof.
+  destruct rk as [[]| |[]]; simpl.
+  - apply reborrowN_lookup_case.
+  - apply reborrowN_lookup_case.
+  - apply reborrowN_visit_freeze_sensitive_case.
+  - apply reborrowN_lookup_case.
+  - apply reborrowN_visit_freeze_sensitive_case.
+Qed.
+
+Lemma retag_ref_Some α cids nxtp l old T rk protector new α' nxtp' :
+  retag_ref α cids nxtp l old T rk protector = Some (new, α', nxtp') →
+  (∀ l', (∀ (i : nat), (i < tsize T)%nat → l' ≠ l +ₗ i) → α' !! l' = α !! l') ∧
+  (∀ i, (i < tsize T)%nat → ∃ stk stk',
+    α !! (l +ₗ i) = Some stk ∧
+    α' !! (l +ₗ i) = Some stk' ∧
+    match rk with
+    | SharedRef | RawRef false =>
+      ∃ b : bool, grant stk old
+                 (mkItem (if b then SharedReadOnly else SharedReadWrite)
+                          new protector) cids = Some stk'
+    | UniqueRef false =>
+      grant stk old (mkItem Unique new protector) cids = Some stk'
+    | UniqueRef true | RawRef true =>
+      grant stk old (mkItem SharedReadWrite new protector) cids = Some stk'
+    end).
+Proof.
+  rewrite /retag_ref. destruct (tsize T) eqn:EqT.
+  - intros. simplify_eq. split; [done|intros; lia].
+  - rewrite -EqT. case reborrow as [α1|] eqn:Eq; [|done]. simpl.
+    intros. simplify_eq. by apply reborrow_Some.
+Qed.
+
+Lemma retag_Some α nxtp c cids l old rk pk T new α' nxtp' :
+  retag α nxtp cids c l old rk pk T = Some (new, α', nxtp') →
+  (∀ l', (∀ (i : nat), (i < tsize T)%nat → l' ≠ l +ₗ i) → α' !! l' = α !! l') ∧
+  match pk, rk with
+  (* Mutable reference *)
+  | RefPtr Mutable, _ =>
+      (∀ i, (i < tsize T)%nat → ∃ stk stk',
+        α !! (l +ₗ i) = Some stk ∧
+        α' !! (l +ₗ i) = Some stk' ∧
+        let protector := adding_protector rk c in
+        let perm := if (is_two_phase rk) then SharedReadWrite else Unique in
+        grant stk old (mkItem perm new protector) cids = Some stk')
+  (* Immutable reference *)
+  | RefPtr Immutable, _ =>
+      (∀ i, (i < tsize T)%nat → ∃ stk stk',
+        α !! (l +ₗ i) = Some stk ∧
+        α' !! (l +ₗ i) = Some stk' ∧
+        let protector := adding_protector rk c in
+        ∃ b : bool, grant stk old
+                   (mkItem (if b then SharedReadOnly else SharedReadWrite)
+                            new protector) cids = Some stk')
+  (* If is both raw ptr and Raw retagging, no protector *)
+  | RawPtr Mutable, RawRt =>
+      (∀ i, (i < tsize T)%nat → ∃ stk stk',
+        α !! (l +ₗ i) = Some stk ∧
+        α' !! (l +ₗ i) = Some stk' ∧
+        grant stk old (mkItem SharedReadWrite new None) cids = Some stk')
+  | RawPtr Immutable, RawRt =>
+      (∀ i, (i < tsize T)%nat → ∃ stk stk',
+        α !! (l +ₗ i) = Some stk ∧
+        α' !! (l +ₗ i) = Some stk' ∧
+        ∃ b : bool, grant stk old
+                 (mkItem (if b then SharedReadOnly else SharedReadWrite)
+                          new None) cids = Some stk')
+  (* Box pointer, no protector *)
+  | BoxPtr, _ =>
+      (∀ i, (i < tsize T)%nat → ∃ stk stk',
+        α !! (l +ₗ i) = Some stk ∧
+        α' !! (l +ₗ i) = Some stk' ∧
+        grant stk old (mkItem Unique new None) cids = Some stk')
+  (* Ignore Raw pointer otherwise *)
+  | RawPtr _, _ => α' = α ∧ nxtp' = nxtp ∧ new = old
+  end.
+Proof.
+  rewrite /retag. destruct (tsize T) as [|n] eqn:ST.
+  { rewrite /retag_ref ST /=.
+    destruct pk as [[]|[]|]; [| |destruct rk|destruct rk|]; intros; simplify_eq;
+      (split; [done| intros; try done; lia]). }
+  rewrite -ST.
+  destruct pk as [[]|[]|]; [destruct rk| |destruct rk|destruct rk|];
+    try apply retag_ref_Some;
+    intros; by simplify_eq.
+Qed.
+
+Lemma retag_Some_dom α nxtp c cids l old rk pk T new α' nxtp'
+  (RK: match pk with | RawPtr _ => rk = RawRt | _ => True end) :
+  retag α nxtp cids c l old rk pk T = Some (new, α', nxtp') →
+  ∀ i, (i < tsize T)%nat → (l +ₗ i) ∈ dom (gset loc) α.
+Proof.
+  intros RT i Lti. rewrite elem_of_dom.
+  destruct (retag_Some _ _ _ _ _ _ _ _ _ _ _ _ RT) as [_ EQ].
+  destruct pk as [[]|[]|]; [| |subst rk..|];
+    specialize (EQ _ Lti) as (?&?&?&_); by eexists.
+Qed.
+
+Lemma retag_Some_Ref α nxtp c cids l old rk T mut new α' nxtp'
+  (NZST: (0 < tsize T)%nat)
+  (FRZ: if mut is Immutable then is_freeze T else True)
+  (N2P: rk ≠ TwoPhase) :
+  retag α nxtp cids c l old rk (RefPtr mut) T = Some (new, α', nxtp') →
+  (∀ i, (i < tsize T)%nat → ∃ stk stk',
+        α !! (l +ₗ i) = Some stk ∧
+        α' !! (l +ₗ i) = Some stk' ∧
+        let protector := adding_protector rk c in
+        let pm := if mut is Immutable then SharedReadOnly else Unique in
+        grant stk old (mkItem pm new protector) cids = Some stk').
+Proof.
+  assert (∃ n, tsize T = S n) as [n EqT].
+  { destruct (tsize T); [lia|by eexists]. }
+  rewrite /retag /retag_ref EqT /=; destruct mut; rewrite -EqT.
+  - rewrite (_: is_two_phase rk = false); [|by destruct rk].
+    case reborrow as [α1|] eqn:RB; [|done]. simpl. intros ?. simplify_eq.
+    by apply reborrowN_lookup_case.
+  - case reborrow as [α1|] eqn:RB; [|done]. simpl. intros ?. simplify_eq.
+    move : RB => /=. rewrite visit_freeze_sensitive_is_freeze; [|done].
+    apply reborrowN_lookup_case.
+Qed.
+
+Lemma grant_access1 stk old new cids stk' :
+  new.(perm) ≠ SharedReadWrite →
+  grant stk old new cids = Some stk' →
+  let kind := if grants new.(perm) AccessWrite then AccessWrite else AccessRead in
+  is_Some (access1 stk kind old cids).
+Proof.
+  intros NSRW. rewrite /grant.
+  case find_granting as [[]|]; [|done].
+  simpl. destruct new.(perm); [|done|..];
+    (case access1; [by eexists|done]).
+Qed.
+
+Lemma grant_singleton_eq (it it': item) old cids stk' :
+  grant [it] old it' cids = Some stk' →
+  old = it.(tg).
+Proof.
+  rewrite /grant. case find_granting as [[n p]|] eqn:GR; [simpl|done].
+  intros _.
+  apply fmap_Some in GR as [[i it1] [FIND ?]]. simplify_eq.
+  move : FIND. simpl. case decide => [MT|//]. intros. simplify_eq.
+  by destruct MT.
+Qed.
+
+Lemma retag_Some_local α nxtp c cids l old rk pk T new α' nxtp' :
+  retag α nxtp cids c l old rk pk T = Some (new, α', nxtp') →
+  ∀ l' t',
+    old ≠ (Tagged t') →
+    α !! l' = Some (init_stack (Tagged t')) →
+    α' !! l' = Some (init_stack (Tagged t')).
+Proof.
+  intros RT l' t' NEQt Eqstk.
+  destruct (retag_Some _ _ _ _ _ _ _ _ _ _ _ _ RT) as [NEQ EQ].
+  destruct (block_case l l' (tsize T)) as [?|(i & Lti & ?)].
+  { by rewrite NEQ. }
+  subst l'.
+  destruct pk as [[]|[]|].
+  - exfalso. specialize (EQ _ Lti) as (stk & stk' & Eq1 & _ & GR).
+    rewrite Eqstk in Eq1. simplify_eq. by apply grant_singleton_eq in GR.
+  - exfalso. specialize (EQ _ Lti) as (stk & stk' & Eq1 & _ & b & GR).
+    rewrite Eqstk in Eq1. simplify_eq. by apply grant_singleton_eq in GR.
+  - destruct rk; try (destruct EQ; by subst α').
+    exfalso. specialize (EQ _ Lti) as (stk & stk' & Eq1 & _ & GR).
+    rewrite Eqstk in Eq1. simplify_eq. by apply grant_singleton_eq in GR.
+  - destruct rk; try (destruct EQ; by subst α').
+    exfalso. specialize (EQ _ Lti) as (stk & stk' & Eq1 & _ & b & GR).
+    rewrite Eqstk in Eq1. simplify_eq. by apply grant_singleton_eq in GR.
+  - exfalso. specialize (EQ _ Lti) as (stk & stk' & Eq1 & _ & GR).
+    rewrite Eqstk in Eq1. simplify_eq. by apply grant_singleton_eq in GR.
+Qed.
+
+Lemma grant_in_SRW stk old it cids stk' it0
+  (SRW: it.(perm) = SharedReadWrite) (NEQ: it ≠ it0) :
+  grant stk old it cids = Some stk' →
+  it0 ∈ stk' → it0 ∈ stk.
+Proof.
+  rewrite /grant. case find_granting as [[n p]|] eqn:FR; [|done].
+  rewrite /= SRW.
+  case find_first_write_incompatible as [n'|] eqn:FI; [|done].
+  rewrite /= => ?. simplify_eq.
+  move => /item_insert_dedup_subseteq /elem_of_cons [//|//].
+Qed.
+
+Lemma grant_in_non_SRW stk old it cids stk' it0
+  (SRW: it.(perm) ≠ SharedReadWrite) (NEQ: it ≠ it0)
+  (ND: it0.(perm) ≠ Disabled) :
+  grant stk old it cids = Some stk' →
+  it0 ∈ stk' → it0 ∈ stk.
+Proof.
+  rewrite /grant. case find_granting as [[n p]|] eqn:FR; [|done].
+  case it.(perm) eqn:Eqp; [|done|..];
+    cbn -[item_insert_dedup];
+    (case access1 as [[n' stk1]|] eqn:ACC; [|done]);
+    cbn -[item_insert_dedup];
+    intros ?; simplify_eq;
+    (move => /item_insert_dedup_subseteq /elem_of_cons [//|//]);
+    intros IN;
+    apply access1_tagged_sublist in ACC;
+    specialize (ACC _ IN) as (it2 & IN2 & HT & HPR & HP); specialize (HP ND).
+    - have ?: it2 = it0. { destruct it2, it0; simpl in *; by subst. }
+      by subst it2.
+    - have ?: it2 = it0. { destruct it2, it0; simpl in *; by subst. }
+      by subst it2.
+    - have ?: it2 = it0. { destruct it2, it0; simpl in *; by subst. }
+      by subst it2.
+Qed.
+
+Lemma grant_in_preserve stk old it cids stk' it0
+  (NEQ: it ≠ it0) (ND: it0.(perm) ≠ Disabled) :
+  grant stk old it cids = Some stk' →
+  it0 ∈ stk' → it0 ∈ stk.
+Proof.
+  case (decide (it.(perm) = SharedReadWrite)) => ?.
+  - by apply grant_in_SRW.
+  - by apply grant_in_non_SRW.
+Qed.
+
+Lemma retag_item_in α nxtp c cids l old rk pk T new α' nxtp' :
+  retag α nxtp cids c l old rk pk T = Some (new, α', nxtp') →
+  ∀ l' stk' t' it',
+    α' !! l' = Some stk' →
+    it' ∈ stk' → it'.(tg) = Tagged t' → it'.(perm) ≠ Disabled →
+    (t' < nxtp)%nat →
+    ∃ stk, α !! l' = Some stk ∧ it' ∈ stk.
+Proof.
+  intros RT l' stk' t' it' Eqstk' In' Eqt' ND' Lt'.
+  destruct (retag_Some _ _ _ _ _ _ _ _ _ _ _ _ RT) as [NEQ EQ].
+  destruct (block_case l l' (tsize T)) as [?|(i & Lti & ?)].
+  { rewrite NEQ // in Eqstk'. naive_solver. }
+  assert (∃ sz, tsize T = S sz) as [sz Eqsz].
+  { destruct (tsize T); [lia|by eexists]. }
+  subst l'.
+  move : RT. rewrite /retag /= /retag_ref Eqsz.
+  destruct pk as [[]|[]|].
+  - specialize (EQ _ Lti) as (stk1 & stk2 & Eq1 & Eq2 & GR). simplify_eq.
+    case reborrow as [α1|]; [|done]. simpl. intros. simplify_eq.
+    exists stk1. split; [done|].
+    move : GR In'.
+    apply grant_in_preserve; [|done].
+    intros ?; subst it'. simpl in Eqt'. simplify_eq. lia.
+  - specialize (EQ _ Lti) as (stk1 & stk2 & Eq1 & Eq2 & b & GR). simplify_eq.
+    case reborrow as [α1|]; [|done]. simpl. intros. simplify_eq.
+    exists stk1. split; [done|].
+    move : GR In'.
+    apply grant_in_preserve; [|done].
+    intros ?; subst it'. simpl in Eqt'. simplify_eq. lia.
+  - destruct rk; [by intros; simplify_eq; naive_solver..|
+                  |intros; simplify_eq; naive_solver].
+    specialize (EQ _ Lti) as (stk1 & stk2 & Eq1 & Eq2 & GR). simplify_eq.
+    case reborrow as [α1|]; [|done]. simpl. intros. simplify_eq.
+    exists stk1. split; [done|].
+    move : GR In'. apply grant_in_SRW; [done|intros ?; by subst it'].
+  - destruct rk; [by intros; simplify_eq; naive_solver..|
+                  |intros; simplify_eq; naive_solver].
+    specialize (EQ _ Lti) as (stk1 & stk2 & Eq1 & Eq2 & b & GR). simplify_eq.
+    case reborrow as [α1|]; [|done]. simpl. intros. simplify_eq.
+    exists stk1. split; [done|].
+    move : GR In'. apply grant_in_preserve; [intros ?; by subst it'|done].
+  - specialize (EQ _ Lti) as (stk1 & stk2 & Eq1 & Eq2 & GR). simplify_eq.
+    case reborrow as [α1|]; [|done]. simpl. intros. simplify_eq.
+    exists stk1. split; [done|].
+    move : GR In'.
+    apply grant_in_preserve; [|done].
+    intros ?; subst it'. simpl in Eqt'. simplify_eq. lia.
+Qed.
+
+(* Lemma item_insert_dedup_lookup stk it i (IS: is_Some (stk !! i)):
+  ∃ j, (item_insert_dedup stk it i) !! j = Some it ∧
+    (j = i ∨ (1 ≤ i ∧ j = i - 1)%nat) ∧
+    (∀ j', (j' < j)%nat → (item_insert_dedup stk it i) !! j' = stk !! j').
+Proof.
+  destruct i as [|i]; simpl.
+  - destruct stk as [|it' stk']; [by destruct IS|]. case decide => [->|?].
+    + exists O. naive_solver.
+    + exists O. split; [done|]. split;[by left| intros; lia].
+  - destruct IS as [it1 Eq1]. rewrite Eq1.
+    destruct (stk !! i) as [it2|] eqn:Eq2; last first.
+    { apply lookup_ge_None_1 in Eq2. apply lookup_lt_Some in Eq1. lia. }
+    case decide => [->|?]; [|case decide => [->|?]].
+    + exists i. split; [done|]. rewrite Nat.sub_0_r. split; [right; lia|done].
+    + exists (S i). split; [done|]. split; [by left|done].
+    + exists (S i). rewrite Nat.sub_0_r. split; last split; [|by left|].
+      * rewrite list_lookup_middle // take_length_le //.
+        by eapply Nat.lt_le_incl, lookup_lt_Some.
+      * intros j' Lt'. rewrite lookup_app_l; [apply lookup_take; lia|].
+        rewrite take_length_le //. by eapply Nat.lt_le_incl, lookup_lt_Some.
+Qed. *)
+
+Lemma find_granting_Some stk kind bor i pi :
+  find_granting stk kind bor = Some (i, pi) →
+  is_Some (stk !! i) ∧
+  ∀ j jt, (j < i)%nat → stk !! j = Some jt →
+  ¬ (grants jt.(perm) kind ∧ jt.(tg) = bor).
+Proof.
+  move => /fmap_Some [[i' pi'] [/list_find_Some_not_earlier [Eq1 [MG LT]] Eq2]].
+  simplify_eq. simpl. split; [by eexists|by apply LT].
+Qed.
+
+Lemma item_insert_dedup_new stk new i (NIN: new ∉ stk) (IS: is_Some (stk !! i)):
+  item_insert_dedup stk new i = take i stk ++ new :: drop i stk.
+Proof.
+  destruct i as [|i]; simpl.
+  - destruct stk as [|it stk]; [done|]. rewrite decide_False //.
+    intros ?. subst. apply NIN. by left.
+  - destruct IS as [its Eqs]. rewrite Eqs.
+    destruct (stk !! i) as [it|] eqn:Eq; last first.
+    { apply lookup_ge_None_1 in Eq. apply lookup_lt_Some in Eqs. lia. }
+    rewrite decide_False; last first.
+    { intros ?. subst. by eapply NIN, elem_of_list_lookup_2. }
+    rewrite decide_False //.
+    intros ?. subst. by eapply NIN, elem_of_list_lookup_2.
+Qed.
+
+Lemma item_insert_dedup_case stk new i :
+   item_insert_dedup stk new i = take i stk ++ new :: drop i stk ∨
+   item_insert_dedup stk new i = stk.
+Proof.
+  (* intros [it Eqit]. *) destruct i as [|i]; simpl.
+  - destruct stk; simpl; [by left|].
+    case decide =>?; [subst new|]; [by right|by left].
+  - destruct (stk !! S i) eqn: Eqit.
+    + have Lt := lookup_lt_Some _ _ _ Eqit.
+      destruct (lookup_lt_is_Some_2 stk i) as [it' Eqit']; [lia|].
+      rewrite Eqit'.
+      case decide => ?; [subst new|]; [by right|].
+      case decide => ?; [subst new|]; [by right|by left].
+    + destruct (stk !! i) eqn: Eqit'; [|by left].
+      case decide => ?; [subst new|]; [by right|by left].
+Qed.
+
+Lemma find_first_write_incompatible_le stk p n :
+  find_first_write_incompatible stk p = Some n →
+  (n ≤ length stk)%nat.
+Proof.
+  destruct p; simpl; [by intros; simplify_eq| |done..].
+  case list_find as [[]|]; intros; simplify_eq; lia.
+Qed.
+
+Lemma find_granting_lt stk kind t n p :
+  find_granting stk kind t = Some (n, p) →
+  (n < length stk)%nat.
+Proof.
+  intros [[n1 p1] [[Eq%lookup_lt_Some MG]%list_find_Some ?]]%fmap_Some.
+  by simplify_eq.
+Qed.
+
+Lemma grant_active_SRO_SRW stk old it cids stk' t
+  (SRW: it.(perm) = SharedReadWrite):
+  grant stk old it cids = Some stk' →
+  t ∈ active_SRO stk → t ∈ active_SRO stk'.
+Proof.
+  rewrite /grant. case find_granting as [[n p]|] eqn:FR; [|done].
+  rewrite /= SRW.
+  case find_first_write_incompatible as [n'|] eqn:FI; [|done].
+  rewrite /= => ?. simplify_eq.
+  destruct (item_insert_dedup_case stk it n') as [EQ|EQ]; rewrite EQ; [|done].
+  rewrite SRW /= in FR. intros IN.
+  have IN' := find_granting_incompatible_active_SRO _ _ _ _ _ IN FR.
+  have IN2 := find_first_write_incompatible_active_SRO _ _ _ FI.
+  have Ltn := find_granting_lt _ _ _ _ _ FR.
+  destruct (IN2 _ IN') as (j & jt & Eqjt & Eqp & Eqt & Lt' & HL).
+  have Eqln: length (take n stk) = n by apply take_length_le; lia.
+  have Len' := find_first_write_incompatible_le _ _ _ FI. rewrite Eqln in Len'.
+  have Eqjt' : stk !! j = Some jt.
+  { rewrite lookup_take // in Eqjt. lia. }
+  apply (active_SRO_elem_of_inv j jt t); [|done|done|].
+  - rewrite lookup_app_l; [by rewrite lookup_take|].
+    rewrite take_length_le //. lia.
+  - intros k kt Ltk.
+    rewrite lookup_app_l; last by (rewrite take_length_le; lia).
+    intros Eqkt. apply (HL _ _ Ltk).
+    rewrite lookup_take; [|lia].
+    rewrite lookup_take in Eqkt; [done|lia].
+Qed.
+
+Lemma grant_active_SRO_non_SRW stk old it cids stk' t pm opro
+  (ND: stack_item_tagged_NoDup stk)
+  (SRW: it.(perm) ≠ SharedReadWrite) (NDIS: it.(perm) ≠ Disabled)
+  (IN': mkItem pm (Tagged t) opro ∈ stk')
+  (NEqt: it.(tg) ≠ Tagged t) :
+  grant stk old it cids = Some stk' →
+  t ∈ active_SRO stk → t ∈ active_SRO stk'.
+Proof.
+  rewrite /grant. case find_granting as [[n p]|] eqn:FR; [|done].
+  case it.(perm) eqn:Eqp; [|done|..|done];
+    cbn -[item_insert_dedup];
+    (case access1 as [[n' stk1]|] eqn:ACC; [|done]);
+    cbn -[item_insert_dedup];
+    intros ?; simplify_eq.
+  - intros Int. exfalso.
+    apply (access1_write_remove_incompatible_active_SRO _ _ _ _ _ _ ND
+            Int ACC pm opro).
+    move : IN' => /item_insert_dedup_subseteq /elem_of_cons [|//].
+    intros. by subst it.
+  - intros Int.
+    have IN'2: mkItem pm (Tagged t) opro ∈ stk1.
+    { move : IN' => /item_insert_dedup_subseteq /elem_of_cons [|//].
+      intros. by subst it. }
+    have IN2:= access1_active_SRO_preserving _ _ _ _ _ _ _ _ _ ND IN'2 ACC Int.
+    destruct (item_insert_dedup_case stk1 it 0) as [EQ|EQ]; rewrite EQ //.
+    apply active_SRO_cons_elem_of. split; [done|by right].
+Qed.
+
+Lemma grant_active_SRO_preserving stk old it cids stk' t pm opro
+  (ND: stack_item_tagged_NoDup stk)
+  (NDIS: it.(perm) ≠ Disabled)
+  (IN': mkItem pm (Tagged t) opro ∈ stk')
+  (NEqt: it.(tg) ≠ Tagged t) :
+  grant stk old it cids = Some stk' →
+  t ∈ active_SRO stk → t ∈ active_SRO stk'.
+Proof.
+  case (decide (it.(perm) = SharedReadWrite)) => ?.
+  - by apply grant_active_SRO_SRW.
+  - by eapply grant_active_SRO_non_SRW.
+Qed.
+
+Lemma retag_item_active_SRO_preserving α nxtp c cids l old rk pk T new α' nxtp' :
+  retag α nxtp cids c l old rk pk T = Some (new, α', nxtp') →
+  ∀ l' t' stk stk' it',
+    stack_item_tagged_NoDup stk →
+    α !! l' = Some stk →
+    α' !! l' = Some stk' →
+    it' ∈ stk → it' ∈ stk' →
+    it'.(tg) = Tagged t' → it'.(perm) ≠ Disabled →
+    (t' < nxtp)%nat →
+    t' ∈ active_SRO stk → t' ∈ active_SRO stk'.
+Proof.
+  intros RT l' t' stk stk' it' ND Eqstk Eqstk' In In' Eqt' ND' Lt'.
+  destruct (retag_Some _ _ _ _ _ _ _ _ _ _ _ _ RT) as [NEQ EQ].
+  destruct (block_case l l' (tsize T)) as [?|(i & Lti & ?)].
+  { rewrite NEQ // in Eqstk'. naive_solver. }
+  assert (∃ sz, tsize T = S sz) as [sz Eqsz].
+  { destruct (tsize T); [lia|by eexists]. }
+  subst l'.
+  have ?: Tagged nxtp ≠ Tagged t' by intros ?; simplify_eq; lia.
+  have ?: mkItem it'.(perm) (Tagged t') it'.(protector) ∈ stk'.
+  { rewrite -Eqt'. by destruct it'. }
+  move : RT. rewrite /retag /= /retag_ref Eqsz.
+  destruct pk as [[]|[]|].
+  - specialize (EQ _ Lti) as (stk1 & stk2 & Eq1 & Eq2 & GR).
+    simplify_eq.
+    case reborrow as [α1|]; [|done]. simpl. intros ?. simplify_eq.
+    move : GR.
+    apply (grant_active_SRO_preserving _ _ _ _ _ _ it'.(perm) it'.(protector) ND);
+      [|done..].
+    simpl. by case is_two_phase.
+  - specialize (EQ _ Lti) as (stk1 & stk2 & Eq1 & Eq2 & b & GR).
+    simplify_eq.
+    case reborrow as [α1|]; [|done]. simpl. intros ?. simplify_eq.
+    move : GR.
+    apply (grant_active_SRO_preserving _ _ _ _ _ _ it'.(perm) it'.(protector) ND);
+      [|done..].
+    simpl. by destruct b.
+  - destruct rk; [by intros; simplify_eq; naive_solver..|
+                  |intros; simplify_eq; naive_solver].
+    specialize (EQ _ Lti) as (stk1 & stk2 & Eq1 & Eq2 & GR). simplify_eq.
+    case reborrow as [α1|]; [|done]. simpl. intros ?. simplify_eq.
+    move : GR.
+    by apply (grant_active_SRO_preserving _ _ _ _ _ _ it'.(perm) it'.(protector) ND).
+  - destruct rk; [by intros; simplify_eq; naive_solver..|
+                  |intros; simplify_eq; naive_solver].
+    specialize (EQ _ Lti) as (stk1 & stk2 & Eq1 & Eq2 & b & GR). simplify_eq.
+    case reborrow as [α1|]; [|done]. simpl. intros ?. simplify_eq.
+    move : GR.
+    apply (grant_active_SRO_preserving _ _ _ _ _ _ it'.(perm) it'.(protector) ND);
+      [|done..].
+    simpl. by destruct b.
+  - specialize (EQ _ Lti) as (stk1 & stk2 & Eq1 & Eq2 & GR). simplify_eq.
+    case reborrow as [α1|]; [|done]. simpl. intros ?. simplify_eq.
+    move : GR.
+    by apply (grant_active_SRO_preserving _ _ _ _ _ _ it'.(perm) it'.(protector) ND).
+Qed.
+
+Lemma is_stack_head_app_l it stk1 stk2 (NN: stk1 ≠ []) :
+  is_stack_head it (stk1 ++ stk2) ↔ is_stack_head it stk1.
+Proof.
+  destruct stk1 as [|i stk1]; [done|].
+  split; intros [? Eq]; inversion Eq; simplify_eq; by eexists.
+Qed.
+
+Lemma grant_head_SRW stk old it cids stk' t pro
+  (SRW: it.(perm) = SharedReadWrite) (NEQ: Tagged t ≠ old) :
+  grant stk old it cids = Some stk' →
+  let it' := (mkItem Unique (Tagged t) pro) in
+  is_stack_head it' stk → is_stack_head it' stk'.
+Proof.
+  rewrite /grant. case find_granting as [[n p]|] eqn:FR; [|done].
+  rewrite /= SRW.
+  case find_first_write_incompatible as [n'|] eqn:FI; [|done].
+  rewrite /= => ?. simplify_eq.
+  destruct (item_insert_dedup_case stk it n') as [EQ|EQ]; rewrite EQ; [|done].
+  rewrite SRW /= in FR. intros IN.
+  have IN' := find_granting_incompatible_head _ _ _ _ _ _ _ _ IN NEQ FR.
+  have IN2 := find_first_write_incompatible_head _ _ _ _ _ _ IN' ltac:(done) FI.
+  have Ltn := find_granting_lt _ _ _ _ _ FR.
+  have Eqln: length (take n stk) = n by apply take_length_le; lia.
+  have Len' := find_first_write_incompatible_le _ _ _ FI. rewrite Eqln in Len'.
+  have ?: take n' stk ≠ [].
+  { destruct stk; [simpl in Ltn; lia|]. destruct n'; [lia|done]. }
+  move : IN. rewrite -{1}(take_drop n' stk).
+  by do 2 rewrite is_stack_head_app_l //.
+Qed.
+
+Lemma grant_head_non_SRW stk old it cids stk' t pro
+  (SRW: it.(perm) ≠ SharedReadWrite) (NDIS: it.(perm) ≠ Disabled)
+  (NEQ: Tagged t ≠ old)
+  (ND: stack_item_tagged_NoDup stk)
+  (NEqt: it.(tg) ≠ Tagged t) :
+  let it' := (mkItem Unique (Tagged t) pro) in
+  it' ∈ stk' →
+  grant stk old it cids = Some stk' →
+  is_stack_head it' stk → is_stack_head it' stk'.
+Proof.
+  intros it' IN'.
+  rewrite /grant. case find_granting as [[n p]|] eqn:FR; [|done].
+  case it.(perm) eqn:Eqp; [|done|..|done];
+    cbn -[item_insert_dedup];
+    (case access1 as [[n' stk1]|] eqn:ACC; [|done]);
+    cbn -[item_insert_dedup];
+    intros ?; simplify_eq.
+  - intros Int.
+    have Int': ∃ pro, is_stack_head (mkItem Unique (Tagged t) pro) stk
+      by eexists.
+    exfalso.
+    apply (access1_write_remove_incompatible_head _ _ _ _ _ _
+            ND Int' ACC NEQ Unique pro).
+    move : IN' => /item_insert_dedup_subseteq /elem_of_cons [|//].
+    intros. by subst it.
+  - intros Int.
+    have IN'2: mkItem Unique (Tagged t) pro ∈ stk1.
+    { move : IN' => /item_insert_dedup_subseteq /elem_of_cons [|//].
+      intros. by subst it. }
+    have Int': ∃ pro, is_stack_head (mkItem Unique (Tagged t) pro) stk
+      by eexists.
+    exfalso.
+    have IN2 := (access1_read_replace_incompatible_head _ _ _ _ _ _
+                  ND Int' ACC NEQ Unique pro IN'2).
+    done.
+Qed.
+
+Lemma grant_head_preserving stk old it cids stk' t pro
+  (NDIS: it.(perm) ≠ Disabled)
+  (NEQ: Tagged t ≠ old)
+  (ND: stack_item_tagged_NoDup stk)
+  (NEqt: it.(tg) ≠ Tagged t) :
+  let it' := (mkItem Unique (Tagged t) pro) in
+  it' ∈ stk' →
+  grant stk old it cids = Some stk' →
+  is_stack_head it' stk → is_stack_head it' stk'.
+Proof.
+  intros it' IN'.
+  case (decide (it.(perm) = SharedReadWrite)) => ?.
+  - by apply grant_head_SRW.
+  - by eapply grant_head_non_SRW.
+Qed.
+
+Lemma retag_item_head_preserving α nxtp c cids l old rk pk T new α' nxtp' :
+  retag α nxtp cids c l old rk pk T = Some (new, α', nxtp') →
+  ∀ l' t' stk stk' pro,
+    stack_item_tagged_NoDup stk →
+    α !! l' = Some stk →
+    α' !! l' = Some stk' →
+    Tagged t' ≠ old →
+    let it' := (mkItem Unique (Tagged t') pro) in
+    it' ∈ stk' →
+    (t' < nxtp)%nat →
+    is_stack_head it' stk → is_stack_head it' stk'.
+Proof.
+  intros RT l' t' stk stk' pro ND Eqstk Eqstk' NEqt it' In' Lt'.
+  destruct (retag_Some _ _ _ _ _ _ _ _ _ _ _ _ RT) as [NEQ EQ].
+  destruct (block_case l l' (tsize T)) as [?|(i & Lti & ?)].
+  { rewrite NEQ // in Eqstk'. naive_solver. }
+  assert (∃ sz, tsize T = S sz) as [sz Eqsz].
+  { destruct (tsize T); [lia|by eexists]. }
+  subst l'.
+  have ?: Tagged nxtp ≠ Tagged t' by intros ?; simplify_eq; lia.
+  move : RT. rewrite /retag /= /retag_ref Eqsz.
+  destruct pk as [[]|[]|].
+  - specialize (EQ _ Lti) as (stk1 & stk2 & Eq1 & Eq2 & GR).
+    simplify_eq.
+    case reborrow as [α1|]; [|done]. simpl. intros ?. simplify_eq.
+    move : GR. eapply grant_head_preserving; eauto.
+    simpl. by case is_two_phase.
+  - specialize (EQ _ Lti) as (stk1 & stk2 & Eq1 & Eq2 & b & GR).
+    simplify_eq.
+    case reborrow as [α1|]; [|done]. simpl. intros ?. simplify_eq.
+    move : GR. eapply grant_head_preserving; eauto.
+    simpl. by destruct b.
+  - destruct rk; [by intros; simplify_eq; naive_solver..|
+                  |intros; simplify_eq; naive_solver].
+    specialize (EQ _ Lti) as (stk1 & stk2 & Eq1 & Eq2 & GR). simplify_eq.
+    case reborrow as [α1|]; [|done]. simpl. intros ?. simplify_eq.
+    move : GR. eapply grant_head_preserving; eauto.
+  - destruct rk; [by intros; simplify_eq; naive_solver..|
+                  |intros; simplify_eq; naive_solver].
+    specialize (EQ _ Lti) as (stk1 & stk2 & Eq1 & Eq2 & b & GR). simplify_eq.
+    case reborrow as [α1|]; [|done]. simpl. intros ?. simplify_eq.
+    move : GR. eapply grant_head_preserving; eauto.
+    simpl. by destruct b.
+  - specialize (EQ _ Lti) as (stk1 & stk2 & Eq1 & Eq2 & GR). simplify_eq.
+    case reborrow as [α1|]; [|done]. simpl. intros ?. simplify_eq.
+    move : GR. eapply grant_head_preserving; eauto.
+Qed.
+
+Lemma grant_active_SRW stk old it cids stk' it'
+  (SRW: it.(perm) = SharedReadWrite) :
+  grant stk old it cids = Some stk' →
+  it' ∈ stk → it' ∈ stk'.
+Proof.
+  rewrite /grant. case find_granting as [[n p]|]; [|done].
+  rewrite /= SRW.
+  case find_first_write_incompatible as [n'|]; [|done].
+  rewrite /= => ?. simplify_eq.
+  destruct (item_insert_dedup_case stk it n') as [EQ|EQ]; rewrite EQ; [|done].
+  rewrite -{1}(take_drop n' stk). set_solver.
+Qed.
+
+Lemma grant_active_non_SRW stk old it cids stk' t pm c
+  (SRW: it.(perm) ≠ SharedReadWrite)
+  (Inc: c ∈ cids) :
+  grant stk old it cids = Some stk' →
+  let it' := mkItem pm t (Some c) in
+  it' ∈ stk → it' ∈ stk'.
+Proof.
+  rewrite /grant. case find_granting as [[n p]|] eqn:FR; [|done].
+  case it.(perm) eqn:Eqp; [|done|..|];
+    cbn -[item_insert_dedup];
+    (case access1 as [[n' stk1]|] eqn:ACC; [|done]);
+    cbn -[item_insert_dedup];
+    intros ?; simplify_eq;
+    move => /(access1_active_preserving _ _ _ _ _ _ ACC _ _ _ Inc);
+    (destruct (item_insert_dedup_case stk1 it O) as [EQ|EQ]; rewrite EQ; [|done]);
+    rewrite -{1}(take_drop 0 stk1); set_solver.
+Qed.
+
+Lemma grant_active_preserving stk old it cids stk' t pm c (Inc: c ∈ cids) :
+  grant stk old it cids = Some stk' →
+  let it' := mkItem pm t (Some c) in
+  it' ∈ stk → it' ∈ stk'.
+Proof.
+  case (decide (it.(perm) = SharedReadWrite)) => ?.
+  - by apply grant_active_SRW.
+  - by eapply grant_active_non_SRW.
+Qed.
+
+Lemma retag_item_active_preserving α nxtp c cids l old rk pk T new α' nxtp' :
+  retag α nxtp cids c l old rk pk T = Some (new, α', nxtp') →
+  ∀ l' stk t' c' pm,
+    α !! l' = Some stk →
+    c' ∈ cids →
+    let it' := mkItem pm t' (Some c') in
+    it' ∈ stk →
+    ∃ stk', α' !! l' = Some stk' ∧ it' ∈ stk'.
+Proof.
+  intros RT l' stk t' c' pm Eqstk Inc' it' IN.
+  destruct (retag_Some _ _ _ _ _ _ _ _ _ _ _ _ RT) as [NEQ EQ].
+  destruct (block_case l l' (tsize T)) as [?|(i & Lti & ?)].
+  { rewrite NEQ //. naive_solver. }
+  assert (∃ sz, tsize T = S sz) as [sz Eqsz].
+  { destruct (tsize T); [lia|by eexists]. }
+  subst l'.
+  move : RT. rewrite /retag /= /retag_ref Eqsz.
+  destruct pk as [[]|[]|].
+  - specialize (EQ _ Lti) as (stk1 & stk2 & Eq1 & Eq2 & GR).
+    simplify_eq.
+    case reborrow as [α1|]; [|done]. simpl. intros ?. simplify_eq.
+    exists stk2. split; [done|].
+    move : Inc' GR IN. by apply grant_active_preserving.
+  - specialize (EQ _ Lti) as (stk1 & stk2 & Eq1 & Eq2 & b & GR).
+    simplify_eq.
+    case reborrow as [α1|]; [|done]. simpl. intros ?. simplify_eq.
+    exists stk2. split; [done|].
+    move : Inc' GR IN. by apply grant_active_preserving.
+  - destruct rk; [by intros; simplify_eq; naive_solver..|
+                  |intros; simplify_eq; naive_solver].
+    specialize (EQ _ Lti) as (stk1 & stk2 & Eq1 & Eq2 & GR). simplify_eq.
+    case reborrow as [α1|]; [|done]. simpl. intros ?. simplify_eq.
+    exists stk2. split; [done|].
+    move : Inc' GR IN. by apply grant_active_preserving.
+  - destruct rk; [by intros; simplify_eq; naive_solver..|
+                  |intros; simplify_eq; naive_solver].
+    specialize (EQ _ Lti) as (stk1 & stk2 & Eq1 & Eq2 & b & GR). simplify_eq.
+    case reborrow as [α1|]; [|done]. simpl. intros ?. simplify_eq.
+    exists stk2. split; [done|].
+    move : Inc' GR IN. by apply grant_active_preserving.
+  - specialize (EQ _ Lti) as (stk1 & stk2 & Eq1 & Eq2 & GR). simplify_eq.
+    case reborrow as [α1|]; [|done]. simpl. intros ?. simplify_eq.
+    exists stk2. split; [done|].
+    move : Inc' GR IN. by apply grant_active_preserving.
+Qed.
+
+Lemma item_insert_dedup_new_elem_of stk new n :
+  new ∈ item_insert_dedup stk new n.
+Proof.
+  destruct n as [|n]; simpl.
+  - destruct stk; simpl.
+    + set_solver.
+    + case decide => ?; [subst; set_solver|set_solver].
+  - case (lookup n) as [?|] eqn:Eq1; case (lookup (S n)) as [?|] eqn:Eq2;
+      [..|set_solver];
+      (case decide => ?; [subst|]).
+    + by eapply elem_of_list_lookup_2.
+    + case decide => ?; [subst|set_solver].
+      by eapply elem_of_list_lookup_2.
+    + by eapply elem_of_list_lookup_2.
+    + set_solver.
+    + by eapply elem_of_list_lookup_2.
+    + set_solver.
+Qed.
+
+Lemma grant_elem_of_SRW stk old new cids stk'
+  (SRW: new.(perm) = SharedReadWrite) :
+  grant stk old new cids = Some stk' → new ∈ stk'.
+Proof.
+  rewrite /grant. case find_granting as [[n1 p1]|]; [|done].
+  rewrite SRW. cbn -[item_insert_dedup].
+  case find_first_write_incompatible as [n2|]; [|done].
+  cbn -[item_insert_dedup]. intros. simplify_eq.
+  by apply item_insert_dedup_new_elem_of.
+Qed.
+
+Lemma grant_elem_of_non_SRW stk old new cids stk'
+  (SRW: new.(perm) ≠ SharedReadWrite) :
+  grant stk old new cids = Some stk' → new ∈ stk'.
+Proof.
+  rewrite /grant. case find_granting as [[n1 p1]|]; [|done].
+  cbn -[item_insert_dedup].
+  destruct new.(perm); [|done|..];
+    (case access1 as [[n2 stk2]|]; [|done]);
+    cbn -[item_insert_dedup]; intros; simplify_eq;
+    by apply item_insert_dedup_new_elem_of.
+Qed.
+
+Lemma grant_elem_of stk old new cids stk' :
+  grant stk old new cids = Some stk' → new ∈ stk'.
+Proof.
+  case (decide (new.(perm) = SharedReadWrite)) => ?.
+  - by apply grant_elem_of_SRW.
+  - by apply grant_elem_of_non_SRW.
+Qed.
+
+Lemma retag_fn_entry_item_active α nxtp c cids l old mut T new α' nxtp' :
+  retag α nxtp cids c l old FnEntry (RefPtr mut) T = Some (new, α', nxtp') →
+  ∀ i, (i < tsize T)%nat → ∃ stk' pm, α' !! (l +ₗ i) = Some stk' ∧
+    mkItem pm new (Some c) ∈ stk' ∧ pm ≠ Disabled.
+Proof.
+  intros RT i Lti.
+  destruct (retag_Some _ _ _ _ _ _ _ _ _ _ _ _ RT) as [_ EQ].
+  assert (∃ sz, tsize T = S sz) as [sz Eqsz].
+  { destruct (tsize T); [lia|by eexists]. }
+  move : RT. rewrite /retag /= /retag_ref Eqsz.
+  destruct mut.
+  - specialize (EQ _ Lti) as (stk1 & stk2 & Eq1 & Eq2 & GR).
+    case reborrow as [α1|]; [|done]. simpl. intros ?. simplify_eq.
+    exists stk2, Unique. split; last split; [done| |done].
+    move : GR. by apply grant_elem_of.
+  - specialize (EQ _ Lti) as (stk1 & stk2 & Eq1 & Eq2 & b & GR).
+    case reborrow as [α1|]; [|done]. simpl. intros ?. simplify_eq.
+    exists stk2, (if b then SharedReadOnly else SharedReadWrite).
+    split; last split; [done| |by destruct b].
+    move : GR. by apply grant_elem_of.
+Qed.
